Initial transition to module system

src/MachineImpl.v
@@ -1,7 +1,7 @@
 Require Import Coq.Lists.List.
 Import List.ListNotations.
 
-From StackSafety Require Import Trace.
+From StackSafety Require Import Trace MachineModule.
 
 Require Import coqutil.Word.Naive.
 Require Import coqutil.Word.Properties.
@@ -32,6 +32,9 @@ From RecordUpdate Require Import RecordSet.
 Import RecordSetNotations.
 
 From QuickChick Require Import QuickChick.
+
+Module RISCV <: Machine.
+
 Axiom exception : forall {A}, string -> A.
 Extract Constant exception =>
   "(fun l ->
@@ -40,7 +43,6 @@ Extract Constant exception =>
     | [] -> s
     | c :: l -> Bytes.set s i c; copy (i+1) l
    in failwith (""Exception: "" ^ Bytes.to_string (copy 0 l)))".
-
 
   Definition Word := MachineInt.
   (* Parameter Word *)
@@ -71,7 +73,7 @@ Extract Constant exception =>
 
   Definition wle (w1 w2: Word) : bool :=
     orb (wlt w1 w2) (weq w1 w2).
-  
+
   (*
     Parameter wplus : Word -> nat -> Word.
     Parameter wminus : Word -> nat -> Word.
@@ -120,6 +122,7 @@ Extract Constant exception =>
 
   (* A Value is a Word. *)
   Definition Value : Type := Word.
+  Definition vtow (v : Value) : Word := v.
 
   (* We use a risc-v machine as our machine state and a view as a map from its
      components to their values. *)
@@ -147,19 +150,19 @@ Extract Constant exception =>
     end.
 
   (* Maybe name this pullback instead *)
-Definition jorp (m : MachineState) (k : Component) (v : Value) : MachineState :=
-  match k with
-  | Mem a =>
-    withMem
-    (unchecked_store_byte_list (word.of_Z a)
-                               (Z32s_to_bytes [v]) (getMem m)) m
-  | Reg r => 
-    withRegs (map.put (getRegs m) r (word.of_Z v)) m
-  | PC =>
-    withPc (word.of_Z v) m
-  end.
+  Definition jorp (m : MachineState) (k : Component) (v : Value) : MachineState :=
+    match k with
+    | Mem a =>
+      withMem
+        (unchecked_store_byte_list (word.of_Z a)
+                                   (Z32s_to_bytes [v]) (getMem m)) m
+    | Reg r => 
+      withRegs (map.put (getRegs m) r (word.of_Z v)) m
+    | PC =>
+      withPc (word.of_Z v) m
+    end.
   
-Definition getComponents (m : MachineState) : list Component :=
+  Definition getComponents (m : MachineState) : list Component :=
     (* PC *)
     let pc := [PC] in
     (* Non-zero registers. *)
@@ -177,10 +180,12 @@ Definition getComponents (m : MachineState) : list Component :=
                        then (Mem z) :: acc else acc) nil 
                     (RiscvMachine.getMem m)) in
     pc ++ regs ++ mem.
-  
+
+  Definition ObsType := unit.
+
   (* Observations are values, or silent (tau) *)
   Inductive Observation : Type := 
-  | Out (w:Value) 
+  | Out (w:ObsType) 
   | Tau. 
 
   Definition w32_eqb (w1 w2 : w32) : bool :=
@@ -231,18 +236,13 @@ Definition getComponents (m : MachineState) : list Component :=
 
   Inductive CodeAnnotation :=
   | call
-  | ret
+  | retrn
   | yield
   | scall (f: MachineState -> Addr -> bool)
   | normal
   .
-
-  Inductive CodeStatus :=
-  | inFun   : FunID -> CodeAnnotation -> CodeStatus
-  | notCode : CodeStatus
-  .
   
-  Definition CodeMap := Addr -> CodeStatus.
+  Definition CodeMap := Addr -> option CodeAnnotation.
 
   (* Stack ID of stack pointer *)
   Definition activeStack (sm: StackMap) (m: MachineState) :
@@ -259,19 +259,6 @@ Definition getComponents (m : MachineState) : list Component :=
     | _, _ => false
     end.
 
-  Definition AnnotationOf (cdm : CodeMap) (a:Addr) : option CodeAnnotation :=
-    match cdm a with
-    | inFun f normal => None
-    | inFun f ann => Some ann
-    | notCode => None
-    end.
-
-  Definition isCode' (cdm : CodeMap) (a:Addr) : bool :=
-    match cdm a with
-    | inFun _ _ => true
-    | notCode => false
-    end.
-
   Definition justRet (mc m: MachineState) : Prop :=
     proj m PC = wplus (proj mc PC) 4 /\ proj m (Reg SP) = proj mc (Reg SP).
 
@@ -283,71 +270,77 @@ Definition getComponents (m : MachineState) : list Component :=
       try solve [left; auto];
       right; intros [? ?]; auto.
   Qed.
+End RISCV.
 
-(* TODO: More interesting state/abstract *)
-Inductive Tag : Type :=
-| Tcall
-| Th1
-| Th2
-| Th3
-| Th4    
-| Tinstr
-| Tpc (n : nat)
-| Tr1
-| Tr2
-| Tr3
-| Tsp
-| Tstack (n : nat)
-.
+Module TagPolicy <: Policy RISCV.
+  Import RISCV.
+  
+  (* TODO: More interesting state/abstract *)
+  Inductive Tag : Type :=
+  | Tcall
+  | Th1
+  | Th2
+  | Th3
+  | Th4    
+  | Tinstr
+  | Tpc (n : nat)
+  | Tr1
+  | Tr2
+  | Tr3
+  | Tsp
+  | Tstack (n : nat)
+  .
 
-Derive Show for Tag.
-Derive Show for InstructionI.
+  Derive Show for Tag.
+  Derive Show for InstructionI.
 
-Definition tag_eqb (t1 t2 :  Tag) : bool :=
-  match t1, t2 with
-  | Tcall, Tcall
-  | Th1, Th1
-  | Th2, Th2
-  | Th3, Th3
-  | Th4, Th4           
-  | Tinstr, Tinstr
-  | Tr1, Tr1
-  | Tr2, Tr2
-  | Tr3, Tr3
-  | Tsp, Tsp => true
-  | Tpc n1, Tpc n2
-  | Tstack n1, Tstack n2 => Nat.eqb n1 n2
-  | _, _ => false
-  end.
+  Definition tag_eqb (t1 t2 :  Tag) : bool :=
+    match t1, t2 with
+    | Tcall, Tcall
+    | Th1, Th1
+    | Th2, Th2
+    | Th3, Th3
+    | Th4, Th4           
+    | Tinstr, Tinstr
+    | Tr1, Tr1
+    | Tr2, Tr2
+    | Tr3, Tr3
+    | Tsp, Tsp => true
+    | Tpc n1, Tpc n2
+    | Tstack n1, Tstack n2 => Nat.eqb n1 n2
+    | _, _ => false
+    end.
 
-Definition tag_neqb (t1 t2 :  Tag) : bool :=
-  negb (tag_eqb t1 t2).
+  Definition tag_neqb (t1 t2 :  Tag) : bool :=
+    negb (tag_eqb t1 t2).
 
-Definition calleeTag : Tag := Th1.
+  Definition calleeTag : Tag := Th1.
+  
+  Definition TagSet : Type := list Tag.
+  Definition TagMap : Type := Zkeyed_map TagSet.
+  
+  Fixpoint TagSet_eqb l1 l2 :=
+    match l1, l2 with
+    | nil,nil => true
+    | cons t1 l1', cons t2 l2' =>
+      andb (tag_eqb t1 t2) (TagSet_eqb l1' l2')
+    | _, _ => false
+    end.
 
-Definition TagSet : Type := list Tag.
-Definition TagMap : Type := Zkeyed_map TagSet.
+  (* Map of memory tags *)
+  Record myPolicyState : Type :=
+    {
+    nextid: nat;
+    pctags: TagSet;
+    regtags: TagMap;
+    memtags: TagMap;
+    }.
 
-Fixpoint TagSet_eqb l1 l2 :=
-  match l1, l2 with
-  | nil,nil => true
-  | cons t1 l1', cons t2 l2' =>
-    andb (tag_eqb t1 t2) (TagSet_eqb l1' l2')
-  | _, _ => false
-  end.
+  Definition PolicyState := myPolicyState.
 
-(* Map of memory tags *)
-Record PolicyState : Type :=
-  {
-  nextid: nat;
-  pctags: TagSet;
-  regtags: TagMap;
-  memtags: TagMap;
-  }.
-
-Instance etaPolicyState : Settable _ :=
-  settable! Build_PolicyState <nextid; pctags; regtags; memtags>.
-
+  Instance etaPolicyState : Settable _ :=
+    settable! Build_myPolicyState <nextid; pctags; regtags; memtags>.
+  
   (* Project what we care about from the RiscV state. *)
   Definition pproj (p:  PolicyState) (k: Component):  TagSet :=
     match k with
@@ -365,452 +358,251 @@ Instance etaPolicyState : Settable _ :=
     end.
 
 
-(* TODO: Rename MPState to State and MPTrace to Trace, mp -> t *)
-Definition MPState : Type := MachineState * PolicyState.
-Definition ms (mp : MPState) := fst mp.
-Definition ps (mp : MPState) := snd mp.
+  (* TODO: Rename MPState to State and MPTrace to Trace, mp -> t *)
+  Definition MPState : Type := MachineState * PolicyState.
+  Definition ms (mp : MPState) := fst mp.
+  Definition ps (mp : MPState) := snd mp.
 
-(* TODO: Real policy. *)
-(* ...
-   TODO: Use [MonadNotations] *)
+  (* TODO: Real policy. *)
+  (* ...
+     TODO: Use [MonadNotations] *)
 
-(* Definition callTags := [Tinstr; Tcall]. *)
+  (* Definition callTags := [Tinstr; Tcall]. *)
 
-(* TODO: Monadic syntax *)
-Definition policyArith (p : PolicyState) (pc : word) (rd rs1 rs2 : Z) : option PolicyState :=
-  tinstr <- map.get (memtags p) (word.unsigned pc);
-  trs1 <- map.get (regtags p) rs1;
-  trs2 <- map.get (regtags p) rs2;
-  trd <- map.get (regtags p) rd;
-  match tinstr, existsb (tag_eqb Tsp) trs1, existsb (tag_eqb Tsp) trs2, trd with
-  | [Tinstr], false, false, [] => Some p
-  | _, _, _, _ => None
-  end.
-
-Definition policyBranch (p : PolicyState) (pc : word) (rs1 rs2 : Z) : option PolicyState :=
-  tinstr <- map.get (memtags p) (word.unsigned pc);
-  trs1 <- map.get (regtags p) rs1;
-  trs2 <- map.get (regtags p) rs2;
-  match tinstr, existsb (tag_eqb Tsp) trs1, existsb (tag_eqb Tsp) trs2 with
-  | [Tinstr], false, false => Some p
-  | _, _, _ => None
-  end.
-
-Definition policyImmArith (p : PolicyState) (pc : word) (rd rs (*imm*) : Z) : option PolicyState :=
-  tinstr <- map.get (memtags p) (word.unsigned pc);
-  let tpc := pctags p in
-  trs <- map.get (regtags p) rs;
-  trd <- map.get (regtags p) rd;
-  match tinstr with
-  | [Tinstr] =>
-    match forallb (tag_neqb Tsp) trs, forallb (tag_neqb Tsp) trd with
-    | true, true => Some (p <| regtags := map.put (regtags p) rd [] |>)
-    | _, _ => None
-    end
-  | [Tinstr; Th1] =>
-    match existsb (tag_eqb Th1) tpc, trs with
-    | true, [Tsp] => Some (p <| pctags := filter (tag_neqb Th1) tpc ++ [Th2] |>
-                             <| regtags := map.put (regtags p) rd [Tsp] |>)
-    | _, _ => None
-    end
-  | [Tinstr; Tr2] =>
-    match existsb (tag_eqb Tr2) tpc, trs with
-    | true, [Tsp] => Some (p <| pctags := filter (tag_neqb Tr2) tpc ++ [Tr3] |>
-                             <| regtags := map.put (regtags p) rd [Tsp] |>)
-    | _, _ => None
-    end
-  | _ => None
-  end.
-
-Definition policyJal (p : PolicyState) (pc : word) (rd : Z) : option PolicyState :=
-  match pctags p, map.get (memtags p) (word.unsigned pc) with
-  | [Tpc old], Some [Tinstr; Tcall] =>
-    let newid := S (nextid p) in (* TODO: This is not next but last! *)
-    Some (p <| nextid := newid |>
-            <| pctags := [Tpc newid; Th1] |>
-            <| regtags := map.put (regtags p) rd [Tpc old] |>)
-  | _, _ => None
-  end.
-
-Definition policyJalr (p : PolicyState) (pc : word) (rd rs : Z) : option PolicyState :=
-  tinstr <- map.get (memtags p) (word.unsigned pc);
-  let tpc := pctags p in
-  ttarget <- map.get (regtags p) rs;
-  treturn <- map.get (regtags p) rd;
-  match tinstr with
-  | [Tinstr] =>
-    match tpc, ttarget, treturn with
-    | [Tpc _], [], [] => Some p
-    | _, _, _ => None
-    end
-  | [Tinstr; Tr3] =>
-    match tpc, ttarget with
-    | [Tpc _; Tr3], [Tpc old] => Some (p <| pctags := [Tpc old] |>
-                                         <| regtags := map.put (regtags p) rd [] |>)
-    | _, _ => None
-    end
-  | _ => None
-  end.
-
-Definition policyLoad (p : PolicyState) (pc rsdata : word) (rd rs imm : Z) : option PolicyState :=
-  tinstr <- map.get (memtags p) (word.unsigned pc);
-  let addr := word.unsigned rsdata + imm in
-  taddr <- map.get (memtags p) addr;
-  let tpc := pctags p in
-  trs <- map.get (regtags p) rs;
-  match tinstr with
-
-  | [Tinstr] =>
-(*    Some (p <| regtags := map.put (regtags p) rd [] |>) (* ERROR *) *)
-
-    match tpc, taddr with
-    | [Tpc pcdepth], [Tstack memdepth] =>
-      if Nat.leb pcdepth memdepth then Some (p <| regtags := map.put (regtags p) rd [] |>)
-      else None
-    | _, _ => None
-    end
-
-  | [Tinstr; Tr1] =>
-    match trs, taddr with
-    | [Tsp], [Tpc _] => Some (p <| pctags := pctags p ++ [Tr2] |>
-                                <| regtags := map.put (regtags p) rd taddr |>)
-    | _, _ => None
-    end
-  | _ => None
-  end.
-
-Definition getdef {T} m k (vdef : T) :=
-  match map.get m k with
-  | Some v => v
-  | None => vdef
-  end.
-
-Definition policyStore (p : PolicyState) (pc rddata : word) (rd rs imm : Z) : option PolicyState :=
-  tinstr <- map.get (memtags p) (word.unsigned pc);
-  let addr := word.unsigned rddata + imm in
-  (* tmem <- map.get (memtags p) addr; *)
-  let tmem := getdef (memtags p) addr [] in
-  let tpc := pctags p in
-  trs <- map.get (regtags p) rs;
-  taddr <- map.get (regtags p) rd;
-  match tinstr with
-  | [Tinstr] =>
-    (* TODO: Relaxed in order for program to work: no stack-indexed writes? *)
-    match tpc, existsb (tag_eqb Tsp) taddr, trs, tmem with
-    | [Tpc depth], (*false*)_, [], [] =>
-        Some (p <| memtags := map.put (memtags p) addr [Tpc depth] |>)
-    | [Tpc depth], (*false*)_, [], [Tpc memdepth] =>
-      if Nat.eqb depth memdepth then  
-        Some (p <| memtags := map.put (memtags p) addr [Tpc depth] |>)
-      else None  
+  (* TODO: Monadic syntax *)
+  Definition policyArith (p : PolicyState) (pc : word) (rd rs1 rs2 : Z) : option PolicyState :=
+    tinstr <- map.get (memtags p) (word.unsigned pc);
+    trs1 <- map.get (regtags p) rs1;
+    trs2 <- map.get (regtags p) rs2;
+    trd <- map.get (regtags p) rd;
+    match tinstr, existsb (tag_eqb Tsp) trs1, existsb (tag_eqb Tsp) trs2, trd with
+    | [Tinstr], false, false, [] => Some p
     | _, _, _, _ => None
-    end
-  | [Tinstr; Th2] =>
-    (*    trace (show (tpc, existsb (tag_eqb Th1) tpc, trs, taddr) ++ nl)%string *)
-    ( 
-    match existsb (tag_eqb Th2) tpc, trs, taddr with
-    | true, cons (Tpc depth) nil, cons Tsp nil =>
-      Some (p <| pctags := filter (tag_neqb Th2) tpc ++ [Th3] |>
-              <| memtags := map.put (memtags p) addr [Tpc depth] |>)
-    | _, _, _ =>
-      None
-    end)
-  | [Tinstr; Th3] =>
-    (* trace (show (tpc, existsb (tag_eqb Th3) tpc, trs, taddr) ++ nl)%string  *)
-    ( 
-    match tpc, taddr with
-    | ([Tpc depth; Th3]), cons Tsp nil =>
-      Some (p <| pctags := filter (tag_neqb Th3) tpc ++ [Th4] |>
-              <| memtags := map.put (memtags p) addr [Tpc depth] |>)
-    | _, _ =>
-      None
-    end)
-  | [Tinstr; Th4] =>
-    (*    trace (show (tpc, existsb (tag_eqb Th1) tpc, trs, taddr) ++ nl)%string *)
-    ( 
-    match tpc, taddr with
-    | ([Tpc depth; Th4]), cons Tsp nil =>
-      Some (p <| pctags := filter (tag_neqb Th4) tpc |>
-              <| memtags := map.put (memtags p) addr [Tpc depth] |>)
-    | _, _ =>
-      None
-    end      
-      )
-  | _ => None
-  end.
-
-Definition decodeI (w : w32) : option InstructionI :=
-  match decode RV32IM (LittleEndian.combine 4 w) with
-  | IInstruction i => Some i
-  | _ => None
-  end.
-
-Definition pstep (mp : MPState) : option PolicyState :=
-  (*  trace ("Entering pstep..." ++ nl)%string *)
-  (
-  let '(m, p) := mp in
-  let pc := getPc m in
-  w <- loadWord (getMem m) pc;
-  i <- decodeI w;
-  match i with
-  | Add  rd rs1 rs2 | Sub rd rs1 rs2 | Sll rd rs1 rs2 | Slt rd rs1 rs2
-  | Sltu rd rs1 rs2 | Xor rd rs1 rs2 | Or  rd rs1 rs2 | Srl rd rs1 rs2
-  | Sra  rd rs1 rs2 | And rd rs1 rs2
-    => policyArith p pc rd rs1 rs2
-  | Beq  rs1 rs2 _ | Bne  rs1 rs2 _ | Blt rs1 rs2 _ | Bge rs1 rs2 _
-  | Bltu rs1 rs2 _ | Bgeu rs1 rs2 _
-    => policyBranch p pc rs1 rs2
-  | Addi rd rs _ | Slti rd rs _ | Sltiu rd rs _ | Xori rd rs _ | Ori rd rs _
-  | Andi rd rs _ | Slli rd rs _ | Srli  rd rs _ | Srai rd rs _
-    => policyImmArith p pc rd rs
-  | Jal rd _
-    => policyJal p pc rd
-  | Jalr rd rs _
-    => policyJalr p pc rd rs
-  | Lb rd rs imm | Lh rd rs imm | Lw rd rs imm | Lbu rd rs imm | Lhu rd rs imm
-    => rsdata <- map.get (getRegs m) rs;
-       policyLoad p pc rsdata rd rs imm
-  | Sb rd rs imm | Sh rd rs imm | Sw rd rs imm
-    => rddata <- map.get (getRegs m) rd;
-       policyStore p pc rddata rd rs imm
-  | _
-    => None
-  end).
-
-Definition mpstep (mp : MPState) : option (MPState * Observation) :=
-  let instr : string := 
-      match loadWord (getMem (ms mp)) (getPc (ms mp)) with
-      | Some w32 =>
-        match decode RV32I (        LittleEndian.combine _ w32)  with
-        | IInstruction inst =>
-          show inst
-        | _ => "<Not inst>"%string
-        end
-      | _ => "<Not inst2>"%string
-      end in
-
-  
-(*  trace ("Entering mpstep with" ++ show (word.unsigned (getPc (ms mp))) ++ " @ " ++ show (pctags (ps mp)) ++ " : " ++ instr ++ nl
-        )%string*)
-        (
-  p' <- pstep mp; 
-  match step (ms mp) with
-  | (m', o) =>
-    if Z.eqb (word.unsigned (getPc (ms mp)))
-             (word.unsigned (getPc m'))
-    then None (* error *)
-    else Some (m', p', o)
-  end
-    )
-.
-
-Axiom mpstepCompat :
-  forall m p o m' p',
-    mpstep (m,p) = Some (m',p',o) ->
-    step m = (m',o).
-
-(* TODO: More interesting well-formedness condition *)
-Definition WFInitMPState (mp:MPState) := True.
-
-(********* Steps and Traces ***********)
-
-Definition MTrace := TraceOf MachineState.
-
-CoFixpoint MTraceOf (M : MachineState) : MTrace :=
-  notfinished M (MTraceOf (fst (step M))).
-
-Definition MPTrace := TraceOf MPState.
-
-CoFixpoint MPTraceOf (mp : MPState) : MPTrace :=
-  match mpstep mp with
-  | None => finished mp
-  | Some (mp',o) => notfinished mp (MPTraceOf mp')
-  end.
-
-Definition MTrace' := TraceOf (MachineState * Observation).
-
-CoFixpoint RunOf (m : MachineState) : MTrace' :=
-  notfinished (m,snd (step m)) (RunOf (fst (step m))).
-
-Definition MPTrace' := TraceOf (MachineState * PolicyState * Observation).
-
-CoFixpoint MPRunOf (mp : MPState) : MPTrace' :=
-  match mpstep mp with
-  | None =>
-    finished (mp,Tau)
-  | Some (mp',o) =>
-    notfinished (mp,o) (MPRunOf mp')
-  end.
-
-(********** Machine Lemmas ************)
-Lemma MTraceOfInf :
-  forall m,
-    infinite (MTraceOf m).
-Proof.  
-  intros m m' H.
-  remember (MTraceOf m) as M.
-  generalize dependent m.
-  induction H; intros m HeqM.
-  - rewrite (idTrace_eq (MTraceOf m)) in HeqM.
-    simpl in *.
-    inversion HeqM.
-  - rewrite (idTrace_eq (MTraceOf m)) in HeqM.
-    simpl in *.
-    inversion HeqM; subst; clear HeqM.
-    eapply IHLast; eauto.
-Qed.
-
-Lemma MPTraceOfHead: forall mp, mp = head (MPTraceOf mp).
-Proof.
-  intros. destruct mp.  simpl. 
-  (* destruct (mpstep (m,p)); auto; destruct p0; auto. *)
-(* Qed. *)
-Abort. (* FIXME *)
-
-(* ******************* Trace stuff ********************* *)
-
-Section WITH_STATE.
-  Variable CtxState : Type.
-  Variable CtxStateUpdate : MachineState -> CtxState -> CtxState.
-  Variable initCtx : MachineState -> CtxState.
-  
-  Definition MPCState : Type := MachineState * PolicyState * CtxState.
-  Definition MPCTrace := TraceOf MPCState.
-  Definition mstate : MPCState -> MachineState := fun '(m,p,cs) => m.
-  Definition pstate : MPCState -> PolicyState := fun '(m,p,cs) => p.
-  Definition cstate : MPCState -> CtxState := fun '(m,p,cs) => cs.
-
-  Definition mpcstep (mpc:MPCState) : option (MPCState * Observation) :=
-    option_map
-      (fun '(m,p,o) => (m,p,CtxStateUpdate (mstate mpc) (cstate mpc),o))
-      (mpstep (mstate mpc,pstate mpc)).
-  
-  Inductive StepsTo : MPCState -> MPCState -> Prop :=
-  | already : forall mpc, StepsTo mpc mpc
-  | future : forall mpc mpc' mpc'' o,
-      StepsTo mpc mpc' ->
-      mpcstep mpc' = Some (mpc'',o) ->
-      StepsTo mpc mpc''.
-
-  Inductive StepsToWhenObs (P:MPCState -> Prop) : MPCState -> MPCState -> TraceOf Observation -> Prop :=
-  | when : forall mpc,
-      P mpc ->
-      StepsToWhenObs P mpc mpc (finished Tau)
-  | futureWhen : forall mpc mpc' mpc'' o O,
-      ~ P mpc ->
-      mpcstep mpc = Some (mpc',o) ->
-      StepsToWhenObs P mpc' mpc'' O ->
-      StepsToWhenObs P mpc mpc'' (notfinished o O).
-
-  Definition StepsToWhen P mpc mpc' := exists O, StepsToWhenObs P mpc mpc' O.
-
-  Inductive FullObsTrace : MPCState -> TraceOf Observation -> Prop :=
-  | stepIt : forall mpc mpc' o O,
-      mpcstep mpc = Some (mpc',o) ->
-      FullObsTrace mpc' O ->
-      FullObsTrace mpc (notfinished o O).
-
-  Definition NeverStepsToObs P mpc O :=
-    FullObsTrace mpc O /\
-    forall mpc',
-      ~ StepsToWhen P mpc mpc'.
-
-  Definition Reachable (mpc:MPCState) : Prop :=
-    exists mpinit,
-      WFInitMPState mpinit /\ StepsTo (mpinit,initCtx (fst mpinit)) mpc.
-
-  CoFixpoint MPCTraceOf (mpc : MPCState) : MPCTrace :=
-    match mpcstep mpc with
-    | None => finished mpc
-    | Some (mpc',o) => notfinished mpc (MPCTraceOf mpc')
     end.
 
-  CoInductive MPCTraceToWhen (P:MPCState -> Prop) : MPCState -> MPCTrace -> Prop :=
-  | TTWNow : forall mpc,
-      P mpc ->
-      MPCTraceToWhen P mpc (finished mpc)
-  | TTWNever : forall mpc,
-      mpcstep mpc = None ->
-      MPCTraceToWhen P mpc (finished mpc)
-  | TTWLater : forall mpc mpc' o MPC,
-      ~ P mpc ->
-      mpcstep mpc = Some (mpc',o) ->
-      MPCTraceToWhen P mpc' MPC ->
-      MPCTraceToWhen P mpc (notfinished mpc MPC)
-  .
-  
-  (* Similarly, with WithObs we relate an MCPTrace into the MPOTrace
-     corresponding to its steps annotated with their observations. We feed
-     each step's observation forward, to line up with the machine state that follows that step.
-     We will need this later. *)
-  Inductive WithObs (o:Observation) : MPCTrace -> TraceOf Observation -> Prop :=
-  | WOFinished : forall mpc,
-      WithObs o (finished mpc) (finished o)
-  | WONotfinished : forall mpc mpc' o' MPC O,
-      WithObs o' MPC O ->
-      mpcstep mpc = Some (mpc',o') ->
-      WithObs o (notfinished mpc MPC) (notfinished o O).
-  
-  (* ObsOfMCP starts the observation with Tau, reflecting that initially
-     there is no observation until a step occurs. *)
-  Definition ObsOfMPC := WithObs Tau.
-  
-  Inductive Segment (f : MPCState -> Prop) : MPCTrace -> MPCTrace -> Prop :=
-  | SegCurrent : forall MPC MPC' mpc,
-      f mpc ->
-      PrefixUpTo (fun mpc' => ~ f mpc') MPC MPC' ->
-      Segment f (notfinished mpc MPC) (notfinished mpc MPC')
-  | SegNot : forall MPC MPCpre MPCsuff MPC' mpc,
-      ~ f mpc ->
-      SplitInclusive f MPC MPCpre MPCsuff ->
-      Segment f MPCsuff MPC' ->
-      Segment f (notfinished mpc MPC) MPC'
-  | SegSkip : forall MPC MPCpre MPCsuff MPC' mpc,
-      f mpc ->
-      SplitInclusive f MPC MPCpre MPCsuff ->
-      Segment f MPCsuff MPC' ->
-      Segment f (notfinished mpc MPC) MPC'
-  .
+  Definition policyBranch (p : PolicyState) (pc : word) (rs1 rs2 : Z) : option PolicyState :=
+    tinstr <- map.get (memtags p) (word.unsigned pc);
+    trs1 <- map.get (regtags p) rs1;
+    trs2 <- map.get (regtags p) rs2;
+    match tinstr, existsb (tag_eqb Tsp) trs1, existsb (tag_eqb Tsp) trs2 with
+    | [Tinstr], false, false => Some p
+    | _, _, _ => None
+    end.
 
-  Definition ReachableSegment (f : MPCState -> Prop) (MPC:MPCTrace) : Prop :=
-    exists mpinit,
-      WFInitMPState mpinit /\ Segment f (MPCTraceOf (mpinit,initCtx (fst mpinit))) MPC.
+  Definition policyImmArith (p : PolicyState) (pc : word) (rd rs (*imm*) : Z) : option PolicyState :=
+    tinstr <- map.get (memtags p) (word.unsigned pc);
+    let tpc := pctags p in
+    trs <- map.get (regtags p) rs;
+    trd <- map.get (regtags p) rd;
+    match tinstr with
+    | [Tinstr] =>
+      match forallb (tag_neqb Tsp) trs, forallb (tag_neqb Tsp) trd with
+      | true, true => Some (p <| regtags := map.put (regtags p) rd [] |>)
+      | _, _ => None
+      end
+    | [Tinstr; Th1] =>
+      match existsb (tag_eqb Th1) tpc, trs with
+      | true, [Tsp] => Some (p <| pctags := filter (tag_neqb Th1) tpc ++ [Th2] |>
+                                                   <| regtags := map.put (regtags p) rd [Tsp] |>)
+      | _, _ => None
+      end
+    | [Tinstr; Tr2] =>
+      match existsb (tag_eqb Tr2) tpc, trs with
+      | true, [Tsp] => Some (p <| pctags := filter (tag_neqb Tr2) tpc ++ [Tr3] |>
+                                                   <| regtags := map.put (regtags p) rd [Tsp] |>)
+      | _, _ => None
+      end
+    | _ => None
+    end.
 
-  Lemma ReachableStepsToWhenSegment :
-    forall mpc mpc' P,
-      Reachable mpc ->
-      StepsToWhen P mpc mpc' ->
-      exists MPC,
-        ReachableSegment P MPC /\
-        head MPC = mpc /\
-        Last MPC mpc'.
-  Proof.
-  Admitted.
-(*    intros. destruct H0 as [O]. induction H0.
-    - exists (finished mpc).
-      split.
-      + unfold ReachableSegment.
-        unfold Reachable in H.
-        destruct H as [mpinit]; exists mpinit.
-        destruct H. split; auto. *)
+  Definition policyJal (p : PolicyState) (pc : word) (rd : Z) : option PolicyState :=
+    match pctags p, map.get (memtags p) (word.unsigned pc) with
+    | [Tpc old], Some [Tinstr; Tcall] =>
+      let newid := S (nextid p) in (* TODO: This is not next but last! *)
+      Some (p <| nextid := newid |>
+              <| pctags := [Tpc newid; Th1] |>
+              <| regtags := map.put (regtags p) rd [Tpc old] |>)
+    | _, _ => None
+    end.
+
+  Definition policyJalr (p : PolicyState) (pc : word) (rd rs : Z) : option PolicyState :=
+    tinstr <- map.get (memtags p) (word.unsigned pc);
+    let tpc := pctags p in
+    ttarget <- map.get (regtags p) rs;
+    treturn <- map.get (regtags p) rd;
+    match tinstr with
+    | [Tinstr] =>
+      match tpc, ttarget, treturn with
+      | [Tpc _], [], [] => Some p
+      | _, _, _ => None
+      end
+    | [Tinstr; Tr3] =>
+      match tpc, ttarget with
+      | [Tpc _; Tr3], [Tpc old] => Some (p <| pctags := [Tpc old] |>
+                                           <| regtags := map.put (regtags p) rd [] |>)
+      | _, _ => None
+      end
+    | _ => None
+    end.
+
+  Definition policyLoad (p : PolicyState) (pc rsdata : word) (rd rs imm : Z) : option PolicyState :=
+    tinstr <- map.get (memtags p) (word.unsigned pc);
+    let addr := word.unsigned rsdata + imm in
+    taddr <- map.get (memtags p) addr;
+    let tpc := pctags p in
+    trs <- map.get (regtags p) rs;
+    match tinstr with
+
+    | [Tinstr] =>
+      (*    Some (p <| regtags := map.put (regtags p) rd [] |>) (* ERROR *) *)
+
+      match tpc, taddr with
+      | [Tpc pcdepth], [Tstack memdepth] =>
+        if Nat.leb pcdepth memdepth then Some (p <| regtags := map.put (regtags p) rd [] |>)
+        else None
+      | _, _ => None
+    end
         
+    | [Tinstr; Tr1] =>
+      match trs, taddr with
+      | [Tsp], [Tpc _] => Some (p <| pctags := pctags p ++ [Tr2] |>
+                                  <| regtags := map.put (regtags p) rd taddr |>)
+      | _, _ => None
+      end
+    | _ => None
+    end.
 
-End WITH_STATE.
+  Definition getdef {T} m k (vdef : T) :=
+    match map.get m k with
+    | Some v => v
+    | None => vdef
+    end.
 
-Arguments Segment {_} _ _ _.
-Arguments ObsOfMPC {_}.
-Arguments MPCState {_}.
-Arguments MPCTrace {_}.
-Arguments cstate {_}.
-Arguments mstate {_}.
-Arguments pstate {_}.
-Arguments Reachable {_} _ _ _.
-Arguments mpcstep {_} _ _.
-Arguments MPCTraceOf {_} _.
-Arguments MPCTraceToWhen {_} _ _ _.
-Arguments StepsToWhenObs {_} _ _ _ _.
-Arguments StepsToWhen {_} _ _ _.
-Arguments ReachableSegment {_} _ _ _.
-Arguments NeverStepsToObs {_} _ _ _.
-Arguments FullObsTrace {_} _ _.
+  Definition policyStore (p : PolicyState) (pc rddata : word) (rd rs imm : Z) : option PolicyState :=
+    tinstr <- map.get (memtags p) (word.unsigned pc);
+    let addr := word.unsigned rddata + imm in
+    (* tmem <- map.get (memtags p) addr; *)
+    let tmem := getdef (memtags p) addr [] in
+    let tpc := pctags p in
+    trs <- map.get (regtags p) rs;
+    taddr <- map.get (regtags p) rd;
+    match tinstr with
+    | [Tinstr] =>
+      (* TODO: Relaxed in order for program to work: no stack-indexed writes? *)
+      match tpc, existsb (tag_eqb Tsp) taddr, trs, tmem with
+      | [Tpc depth], (*false*)_, [], [] =>
+        Some (p <| memtags := map.put (memtags p) addr [Tpc depth] |>)
+      | [Tpc depth], (*false*)_, [], [Tpc memdepth] =>
+        if Nat.eqb depth memdepth then  
+          Some (p <| memtags := map.put (memtags p) addr [Tpc depth] |>)
+        else None  
+      | _, _, _, _ => None
+      end
+    | [Tinstr; Th2] =>
+      (*    trace (show (tpc, existsb (tag_eqb Th1) tpc, trs, taddr) ++ nl)%string *)
+      ( 
+        match existsb (tag_eqb Th2) tpc, trs, taddr with
+        | true, cons (Tpc depth) nil, cons Tsp nil =>
+          Some (p <| pctags := filter (tag_neqb Th2) tpc ++ [Th3] |>
+                  <| memtags := map.put (memtags p) addr [Tpc depth] |>)
+        | _, _, _ =>
+          None
+        end)
+    | [Tinstr; Th3] =>
+      (* trace (show (tpc, existsb (tag_eqb Th3) tpc, trs, taddr) ++ nl)%string  *)
+      ( 
+        match tpc, taddr with
+        | ([Tpc depth; Th3]), cons Tsp nil =>
+          Some (p <| pctags := filter (tag_neqb Th3) tpc ++ [Th4] |>
+                  <| memtags := map.put (memtags p) addr [Tpc depth] |>)
+        | _, _ =>
+          None
+        end)
+    | [Tinstr; Th4] =>
+      (*    trace (show (tpc, existsb (tag_eqb Th1) tpc, trs, taddr) ++ nl)%string *)
+      ( 
+        match tpc, taddr with
+        | ([Tpc depth; Th4]), cons Tsp nil =>
+          Some (p <| pctags := filter (tag_neqb Th4) tpc |>
+                  <| memtags := map.put (memtags p) addr [Tpc depth] |>)
+        | _, _ =>
+          None
+        end      
+      )
+    | _ => None
+    end.
+  
+  Definition decodeI (w : w32) : option InstructionI :=
+    match decode RV32IM (LittleEndian.combine 4 w) with
+    | IInstruction i => Some i
+    | _ => None
+    end.
 
+  Definition pstep (mp : MPState) : option PolicyState :=
+    (*  trace ("Entering pstep..." ++ nl)%string *)
+    (
+      let '(m, p) := mp in
+      let pc := getPc m in
+      w <- loadWord (getMem m) pc;
+    i <- decodeI w;
+    match i with
+    | Add  rd rs1 rs2 | Sub rd rs1 rs2 | Sll rd rs1 rs2 | Slt rd rs1 rs2
+    | Sltu rd rs1 rs2 | Xor rd rs1 rs2 | Or  rd rs1 rs2 | Srl rd rs1 rs2
+    | Sra  rd rs1 rs2 | And rd rs1 rs2
+                        => policyArith p pc rd rs1 rs2
+    | Beq  rs1 rs2 _ | Bne  rs1 rs2 _ | Blt rs1 rs2 _ | Bge rs1 rs2 _
+    | Bltu rs1 rs2 _ | Bgeu rs1 rs2 _
+                       => policyBranch p pc rs1 rs2
+    | Addi rd rs _ | Slti rd rs _ | Sltiu rd rs _ | Xori rd rs _ | Ori rd rs _
+    | Andi rd rs _ | Slli rd rs _ | Srli  rd rs _ | Srai rd rs _
+                                                    => policyImmArith p pc rd rs
+    | Jal rd _
+      => policyJal p pc rd
+    | Jalr rd rs _
+      => policyJalr p pc rd rs
+    | Lb rd rs imm | Lh rd rs imm | Lw rd rs imm | Lbu rd rs imm | Lhu rd rs imm
+                                                                   => rsdata <- map.get (getRegs m) rs;
+    policyLoad p pc rsdata rd rs imm
+    | Sb rd rs imm | Sh rd rs imm | Sw rd rs imm
+                                    => rddata <- map.get (getRegs m) rd;
+    policyStore p pc rddata rd rs imm
+    | _
+      => None
+      end).
+
+  Definition mpstep (mp : MPState) : option (MPState * Observation) :=
+    let instr : string := 
+        match loadWord (getMem (ms mp)) (getPc (ms mp)) with
+        | Some w32 =>
+          match decode RV32I (        LittleEndian.combine _ w32)  with
+          | IInstruction inst =>
+            show inst
+          | _ => "<Not inst>"%string
+          end
+        | _ => "<Not inst2>"%string
+        end in
+    
+  
+    (*  trace ("Entering mpstep with" ++ show (word.unsigned (getPc (ms mp))) ++ " @ " ++ show (pctags (ps mp)) ++ " : " ++ instr ++ nl
+        )%string*)
+    (
+      p' <- pstep mp; 
+    match step (ms mp) with
+    | (m', o) =>
+      if Z.eqb (word.unsigned (getPc (ms mp)))
+               (word.unsigned (getPc m'))
+      then None (* error *)
+      else Some (m', p', o)
+    end
+    )
+  .
+
+  Axiom mpstepCompat :
+    forall m p o m' p',
+      mpstep (m,p) = Some (m',p',o) ->
+      step m = (m',o).
+
+
+  (* TODO: More interesting well-formedness condition *)
+  Definition WFInitMPState (mp:MPState) := True.
+End TagPolicy.
