src/MachineModule.v
@@ -1,0 +1,320 @@
+Require Import Coq.Lists.List.
+Import List.ListNotations.
+
+From StackSafety Require Import Trace.
+
+Module Type Machine.
+
+(*  Axiom exception : forall {A}, string -> A.
+  Extract Constant exception =>
+  "(fun l ->
+         let s = Bytes.create (List.length l) in
+          let rec copy i = function
+          | [] -> s
+          | c :: l -> Bytes.set s i c; copy (i+1) l
+          in failwith (""Exception: "" ^ Bytes.to_string (copy 0 l)))". *)
+
+
+  Parameter Word : Type.
+
+  Parameter wlt : Word -> Word -> bool.
+
+  Parameter weq : Word -> Word -> bool.
+
+  Parameter WordEqDec : forall (w1 w2 : Word), {w1 = w2} + {w1 <> w2}.
+
+  Parameter weq_implies_eq :
+    forall w1 w2,
+      weq w1 w2 = true -> w1 = w2.
+
+  Parameter not_weq_implies_neq :
+    forall w1 w2,
+      weq w1 w2 = false -> w1 <> w2.
+
+  Parameter wle : Word -> Word -> bool.
+  
+  Parameter wplus : Word -> nat -> Word.
+
+  Parameter wminus : Word -> nat -> Word.
+
+  Parameter wplus_neq : forall w (n : nat),
+      (n > O)%nat -> w <> wplus w n.
+
+  Definition Addr := Word.
+
+  Parameter Register : Type.
+
+  Parameter RA : Register.
+  Parameter SP : Register.
+  Parameter regEq : Register -> Register -> bool.
+  
+  Inductive Component:=
+  | Mem (a:Addr)
+  | Reg (r:Register)
+  | PC.
+
+  Parameter keqb : Component -> Component -> bool.
+
+  Parameter Value : Type.
+  Parameter vtow : Value -> Word.
+
+  Parameter MachineState : Type.
+  Definition View := Component -> Value.
+
+  Parameter proj : MachineState -> Component -> Value.
+
+  (* Maybe name this pullback instead *)
+  Parameter jorp : MachineState -> Component -> Value -> MachineState.
+  
+  Parameter getComponents : MachineState -> list Component.
+  
+  (* Observations are ObsType, or silent (tau) *)
+  Parameter ObsType : Type.
+  
+  Inductive Observation : Type := 
+  | Out (o:ObsType) 
+  | Tau. 
+
+  (* A Machine State can step to a new Machine State plus an Observation. *)
+  Parameter step : MachineState -> MachineState * Observation.
+
+  Parameter FunID : Type.
+  Parameter StackID : Type.
+
+  (*Definition EntryMap := Addr -> bool.*)
+
+  Definition StackMap := Addr -> option StackID.
+
+  Inductive CodeAnnotation : Type :=
+  | call
+  | retrn
+  | yield
+  | scall (f: MachineState -> Addr -> bool)
+  | normal
+  .
+
+(*  Inductive CodeStatus :=
+  | inFun   : FunID -> CodeAnnotation -> CodeStatus
+  | notCode : CodeStatus
+  .*)
+  
+  Definition CodeMap := Addr -> option CodeAnnotation.
+
+  Parameter activeStack : StackMap -> MachineState -> option StackID.
+   
+  Parameter stack_eqb : StackID -> StackID -> bool.
+
+  Parameter optstack_eqb : option StackID -> option StackID -> bool.
+
+  Parameter justRet : MachineState -> MachineState -> Prop.
+
+  Parameter justRet_dec : forall mc m, {justRet mc m} + {~ justRet mc m}.
+End Machine.
+
+Module Type Policy(M:Machine).
+  Import M.
+
+  Parameter PolicyState : Type.
+
+  (* TODO: Rename MPState to State and MPTrace to Trace, mp -> t *)
+  Definition MPState : Type := MachineState * PolicyState.
+
+  Parameter pstep : MPState -> option PolicyState.
+
+  Parameter mpstep : MPState -> option (MPState * Observation).
+
+  Parameter mpstepCompat :
+    forall m p o m' p',
+      mpstep (m,p) = Some (m',p',o) ->
+      step m = (m',o).
+
+  Parameter WFInitMPState : MPState -> Prop.
+
+End Policy.
+
+Module Type Ctx (M:Machine).
+  Import M.
+
+  Parameter CtxState : Type.
+  Parameter CtxStateUpdate : MachineState -> CtxState -> CtxState.
+  Parameter initCtx : MachineState -> CtxState.
+End Ctx.
+
+Module Type MapMaker (M : Machine).
+  Import M.
+
+  Parameter cdm : CodeMap.
+  Parameter sm : StackMap.
+End MapMaker.
+
+Module MPC (M:Machine) (P:Policy M) (C:Ctx M).
+  Import M.
+  Import P.
+  Import C.
+         
+  Definition MPCState : Type := MachineState * PolicyState * CtxState.
+  Definition MPCTrace := TraceOf MPCState.
+  Definition mstate : MPCState -> MachineState := fun '(m,p,cs) => m.
+  Definition pstate : MPCState -> PolicyState := fun '(m,p,cs) => p.
+  Definition cstate : MPCState -> CtxState := fun '(m,p,cs) => cs.
+  
+  (********** Machine Lemmas ************)
+  (* TODO: redo for MPCTraces *)
+  (*Lemma MTraceOfInf :
+    forall m,
+      infinite (MTraceOf m).
+  Proof.  
+    intros m m' H.
+    remember (MTraceOf m) as M.
+    generalize dependent m.
+    induction H; intros m HeqM.
+    - rewrite (idTrace_eq (MTraceOf m)) in HeqM.
+      simpl in *.
+      inversion HeqM.
+    - rewrite (idTrace_eq (MTraceOf m)) in HeqM.
+      simpl in *.
+      inversion HeqM; subst; clear HeqM.
+      eapply IHLast; eauto.
+  Qed.
+
+ Lemma MPTraceOfHead: forall mp, mp = head (MPTraceOf mp).
+  Proof.
+    intros. destruct mp.  simpl. 
+    (* destruct (mpstep (m,p)); auto; destruct p0; auto. *)
+    (* Qed. *)
+  Abort. (* FIXME *) *)
+
+  Definition mpcstep (mpc:MPCState) : option (MPCState * Observation) :=
+    option_map
+      (fun '(m,p,o) => (m,p,CtxStateUpdate (mstate mpc) (cstate mpc),o))
+      (mpstep (mstate mpc,pstate mpc)).
+  
+  Inductive StepsTo : MPCState -> MPCState -> Prop :=
+  | already : forall mpc, StepsTo mpc mpc
+  | future : forall mpc mpc' mpc'' o,
+      StepsTo mpc mpc' ->
+      mpcstep mpc' = Some (mpc'',o) ->
+      StepsTo mpc mpc''.
+
+  Inductive StepsToWhenObs (P:MPCState -> Prop)
+    : MPCState -> MPCState -> TraceOf Observation -> Prop :=
+  | when : forall mpc,
+      P mpc ->
+      StepsToWhenObs P mpc mpc (finished Tau)
+  | futureWhen : forall mpc mpc' mpc'' o O,
+      ~ P mpc ->
+      mpcstep mpc = Some (mpc',o) ->
+      StepsToWhenObs P mpc' mpc'' O ->
+      StepsToWhenObs P mpc mpc'' (notfinished o O).
+
+  Definition StepsToWhen P mpc mpc' := exists O, StepsToWhenObs P mpc mpc' O.
+
+  Inductive FullObsTrace : MPCState -> TraceOf Observation -> Prop :=
+  | stepIt : forall mpc mpc' o O,
+      mpcstep mpc = Some (mpc',o) ->
+      FullObsTrace mpc' O ->
+      FullObsTrace mpc (notfinished o O).
+
+  Definition NeverStepsToObs P mpc O :=
+    FullObsTrace mpc O /\
+    forall mpc',
+      ~ StepsToWhen P mpc mpc'.
+
+  Definition Reachable (mpc:MPCState) : Prop :=
+    exists mpinit,
+      WFInitMPState mpinit /\ StepsTo (mpinit,initCtx (fst mpinit)) mpc.
+
+  CoFixpoint MPCTraceOf (mpc : MPCState) : MPCTrace :=
+    match mpcstep mpc with
+    | None => finished mpc
+    | Some (mpc',o) => notfinished mpc (MPCTraceOf mpc')
+    end.
+
+  CoInductive MPCTraceToWhen (P:MPCState -> Prop) : MPCState -> MPCTrace -> Prop :=
+  | TTWNow : forall mpc,
+      P mpc ->
+      MPCTraceToWhen P mpc (finished mpc)
+  | TTWNever : forall mpc,
+      mpcstep mpc = None ->
+      MPCTraceToWhen P mpc (finished mpc)
+  | TTWLater : forall mpc mpc' o MPC,
+      ~ P mpc ->
+      mpcstep mpc = Some (mpc',o) ->
+      MPCTraceToWhen P mpc' MPC ->
+      MPCTraceToWhen P mpc (notfinished mpc MPC)
+  .
+  
+  (* Similarly, with WithObs we relate an MCPTrace into the MPOTrace
+     corresponding to its steps annotated with their observations. We feed
+     each step's observation forward, to line up with the machine state that follows that step.
+     We will need this later. *)
+  Inductive WithObs (o:Observation) : MPCTrace -> TraceOf Observation -> Prop :=
+  | WOFinished : forall mpc,
+      WithObs o (finished mpc) (finished o)
+  | WONotfinished : forall mpc mpc' o' MPC O,
+      WithObs o' MPC O ->
+      mpcstep mpc = Some (mpc',o') ->
+      WithObs o (notfinished mpc MPC) (notfinished o O).
+  
+  (* ObsOfMCP starts the observation with Tau, reflecting that initially
+     there is no observation until a step occurs. *)
+  Definition ObsOfMPC := WithObs Tau.
+  
+  Inductive Segment (f : MPCState -> Prop) : MPCTrace -> MPCTrace -> Prop :=
+  | SegCurrent : forall MPC MPC' mpc,
+      f mpc ->
+      PrefixUpTo (fun mpc' => ~ f mpc') MPC MPC' ->
+      Segment f (notfinished mpc MPC) (notfinished mpc MPC')
+  | SegNot : forall MPC MPCpre MPCsuff MPC' mpc,
+      ~ f mpc ->
+      SplitInclusive f MPC MPCpre MPCsuff ->
+      Segment f MPCsuff MPC' ->
+      Segment f (notfinished mpc MPC) MPC'
+  | SegSkip : forall MPC MPCpre MPCsuff MPC' mpc,
+      f mpc ->
+      SplitInclusive f MPC MPCpre MPCsuff ->
+      Segment f MPCsuff MPC' ->
+      Segment f (notfinished mpc MPC) MPC'
+  .
+
+  Definition ReachableSegment (f : MPCState -> Prop) (MPC:MPCTrace) : Prop :=
+    exists mpinit,
+      WFInitMPState mpinit /\ Segment f (MPCTraceOf (mpinit,initCtx (fst mpinit))) MPC.
+
+  Lemma ReachableStepsToWhenSegment :
+    forall mpc mpc' P,
+      Reachable mpc ->
+      StepsToWhen P mpc mpc' ->
+      exists MPC,
+        ReachableSegment P MPC /\
+        head MPC = mpc /\
+        Last MPC mpc'.
+  Proof.
+  Admitted.
+(*    intros. destruct H0 as [O]. induction H0.
+    - exists (finished mpc).
+      split.
+      + unfold ReachableSegment.
+        unfold Reachable in H.
+        destruct H as [mpinit]; exists mpinit.
+        destruct H. split; auto. *)
+        
+End MPC.
+
+(*Arguments Segment {_} _ _ _.
+Arguments ObsOfMPC {_}.
+Arguments MPCState {_}.
+Arguments MPCTrace {_}.
+Arguments cstate {_}.
+Arguments mstate {_}.
+Arguments pstate {_}.
+Arguments Reachable {_} _ _ _.
+Arguments mpcstep {_} _ _.
+Arguments MPCTraceOf {_} _.
+Arguments MPCTraceToWhen {_} _ _ _.
+Arguments StepsToWhenObs {_} _ _ _ _.
+Arguments StepsToWhen {_} _ _ _.
+Arguments ReachableSegment {_} _ _ _.
+Arguments NeverStepsToObs {_} _ _ _.
+Arguments FullObsTrace {_} _ _. *)
+
