src/ObsTrace.v
@@ -1,64 +1,68 @@
-From StackSafety Require Import Trace MachineImpl.
+From StackSafety Require Import Trace MachineModule.
 
+Module ObsTrace (M:Machine).
+  Import M.
 
   Definition ObsTrace := TraceOf Observation.
 
-Ltac app_frobber :=
-  repeat match goal with
-         | |- context[(finished ?T) ^ ?OT] =>
-           rewrite (idTrace_eq (finished T ^ OT)); simpl
-         | |- context[(notfinished ?O ?T) ^ ?OT] =>
-           rewrite (idTrace_eq (notfinished O T ^ OT)); simpl
-         | [H: context[(finished ?T) ^ ?OT] |- _ ] =>
-           rewrite (idTrace_eq (finished T ^ OT)) in H; simpl in H
-         | [H: context[(notfinished ?O ?T) ^ ?OT] |- _ ] =>
-           rewrite (idTrace_eq (notfinished O T ^ OT)) in H; simpl in H
-         end.
+  Ltac app_frobber :=
+    repeat match goal with
+           | |- context[(finished ?T) ^ ?OT] =>
+             rewrite (idTrace_eq (finished T ^ OT)); simpl
+           | |- context[(notfinished ?O ?T) ^ ?OT] =>
+             rewrite (idTrace_eq (notfinished O T ^ OT)); simpl
+           | [H: context[(finished ?T) ^ ?OT] |- _ ] =>
+             rewrite (idTrace_eq (finished T ^ OT)) in H; simpl in H
+           | [H: context[(notfinished ?O ?T) ^ ?OT] |- _ ] =>
+             rewrite (idTrace_eq (notfinished O T ^ OT)) in H; simpl in H
+           end.
 
-Ltac join_frobber :=
-  repeat match goal with
-         | |- context[(finished ?T) ^^ ?OT] =>
-           rewrite (idTrace_eq (finished T ^^ OT)); simpl
-         | |- context[(notfinished ?O ?T) ^^ ?OT] =>
-           rewrite (idTrace_eq (notfinished O T ^^ OT)); simpl
-         | [H: context[(finished ?T) ^^ ?OT] |- _ ] =>
-           rewrite (idTrace_eq (finished T ^^ OT)) in H; simpl in H
-         | [H: context[(notfinished ?O ?T) ^^ ?OT] |- _ ] =>
-           rewrite (idTrace_eq (notfinished O T ^^ OT)) in H; simpl in H
-         end.
+  Ltac join_frobber :=
+    repeat match goal with
+           | |- context[(finished ?T) ^^ ?OT] =>
+             rewrite (idTrace_eq (finished T ^^ OT)); simpl
+           | |- context[(notfinished ?O ?T) ^^ ?OT] =>
+             rewrite (idTrace_eq (notfinished O T ^^ OT)); simpl
+           | [H: context[(finished ?T) ^^ ?OT] |- _ ] =>
+             rewrite (idTrace_eq (finished T ^^ OT)) in H; simpl in H
+           | [H: context[(notfinished ?O ?T) ^^ ?OT] |- _ ] =>
+             rewrite (idTrace_eq (notfinished O T ^^ OT)) in H; simpl in H
+           end.
 
-Ltac maptrace_frobber :=
-  repeat match goal with
-         | |- context[mapTrace ?f (finished ?t)] =>
-           rewrite (idTrace_eq (mapTrace f (finished t))); unfold mapTrace; simpl
-         | |- context[mapTrace ?f (notfinished ?t ?T)] =>
-           rewrite (idTrace_eq (mapTrace f (notfinished t T))); unfold mapTrace; simpl
-         end.
+  Ltac maptrace_frobber :=
+    repeat match goal with
+           | |- context[mapTrace ?f (finished ?t)] =>
+             rewrite (idTrace_eq (mapTrace f (finished t))); unfold mapTrace; simpl
+           | |- context[mapTrace ?f (notfinished ?t ?T)] =>
+             rewrite (idTrace_eq (mapTrace f (notfinished t T))); unfold mapTrace; simpl
+           end.
 
-(********************** ObsTrace Equivalence *************************)
+  (********************** ObsTrace Equivalence *************************)
 
-CoInductive ObsTraceEq(*_gen R*) : TraceOf Observation -> TraceOf Observation -> Prop :=
-| ObsEqTau1 : forall OO OO'
-                     (HR : (*R*)ObsTraceEq OO OO' : Prop),
-    ObsTraceEq(*_gen R*) (notfinished Tau OO) OO'
-| ObsEqTau2 : forall OO OO'
-                     (HR : (*R*)ObsTraceEq OO OO' : Prop),
-    ObsTraceEq(*_gen R*) OO (notfinished Tau OO')
-| ObsEqNow : forall w OO OO'
-                     (HR : (*R*)ObsTraceEq OO OO' : Prop),
-    ObsTraceEq(*_gen R*) (notfinished (Out w) OO) (notfinished (Out w) OO')
-(*
-| ObsEqFinishedOut : forall w,
-    ObsTraceEq(*_gen R*) (finished (Out w)) (finished (Out w))
-| ObsEqFinishedTau :
-    ObsTraceEq(*_gen R*) (finished Tau) (finished Tau)
- *)
-(* The last thing we need is a way of handling *all-tau* traces.
-   There are a couple of ways of doing that, not sure what will
+  CoInductive ObsTraceEq(*_gen R*) : TraceOf Observation -> TraceOf Observation -> Prop :=
+  | ObsEqTau1 : forall OO OO'
+                       (HR : (*R*)ObsTraceEq OO OO' : Prop),
+      ObsTraceEq(*_gen R*) (notfinished Tau OO) OO'
+  | ObsEqTau2 : forall OO OO'
+                       (HR : (*R*)ObsTraceEq OO OO' : Prop),
+      ObsTraceEq(*_gen R*) OO (notfinished Tau OO')
+  | ObsEqNow : forall o OO OO'
+                      (HR : (*R*)ObsTraceEq OO OO' : Prop),
+      ObsTraceEq(*_gen R*) (notfinished (Out o) OO) (notfinished (Out o) OO')
+  (*
+    | ObsEqFinishedOut : forall w,
+      ObsTraceEq(*_gen R*) (finished (Out w)) (finished (Out w))
+    | ObsEqFinishedTau :
+      ObsTraceEq(*_gen R*) (finished Tau) (finished Tau)
+   *)
+  (* The last thing we need is a way of handling *all-tau* traces.
+     There are a couple of ways of doing that, not sure what will
    play better in proofs. *)
-| ObsEqAllSame : forall OO,
-     ObsTraceEq(*_gen R*) OO OO.
-(* APT: Establishing equality between traces seems hard, and this overlaps
+  | ObsEqAllSame : forall OO,
+      ObsTraceEq(*_gen R*) OO OO.
+
+
+  (* APT: Establishing equality between traces seems hard, and this overlaps
 the previous two cases.  Maybe try:
    ForallTrace (fun o => o = Tau) OO ->
    ForallTrace (fun o => o = Tau) OO' ->
@@ -67,162 +71,162 @@ the previous two cases.  Maybe try:
 LEO: That was the other thing I had in mind. I'll see what makes proofs easier.
 (Note that this proposal overlaps with the first two cases, as well as the last one.)
  *)
-Hint Constructors ObsTraceEq(*_gen*) : core.
+  Hint Constructors ObsTraceEq(*_gen*) : core.
 
-(* Definition ObsTraceEq (OO OO' : TraceOf Observation) := *)
-(*   paco2 ObsTraceEq_gen bot2 OO OO'. *)
-(* Hint Unfold ObsTraceEq : core. *)
-(* Lemma ObsTraceEq_mon : monotone2 ObsTraceEq_gen. Proof. pmonauto. Qed. *)
-(* Hint Resolve ObsTraceEq_mon : paco. *)
+  (* Definition ObsTraceEq (OO OO' : TraceOf Observation) := *)
+  (*   paco2 ObsTraceEq_gen bot2 OO OO'. *)
+  (* Hint Unfold ObsTraceEq : core. *)
+  (* Lemma ObsTraceEq_mon : monotone2 ObsTraceEq_gen. Proof. pmonauto. Qed. *)
+  (* Hint Resolve ObsTraceEq_mon : paco. *)
 
-Notation "OO' ~=_O OO" := (ObsTraceEq OO' OO) (at level 80).
+  Notation "OO' ~=_O OO" := (ObsTraceEq OO' OO) (at level 80).
 
-Lemma ObsTraceEq_sym :
-  forall O O',
-    ObsTraceEq O O' -> ObsTraceEq O' O.
-Proof.
-  cofix COFIX.
-  intros O O' H(*; pfold*).
-  inv H;
-    try (constructor; ((*right;*) apply COFIX; auto) || ((*left;*) auto)).
+  Lemma ObsTraceEq_sym :
+    forall O O',
+      ObsTraceEq O O' -> ObsTraceEq O' O.
+  Proof.
+    cofix COFIX.
+    intros O O' H(*; pfold*).
+    inv H;
+      try (constructor; ((*right;*) apply COFIX; auto) || ((*left;*) auto)).
     (* Or, simplified, [constructor; auto]. *)
-Qed.
+  Qed.
 
-Lemma ObsTraceEqRemoveTau1 :
-  forall T T', ObsTraceEq (notfinished Tau T) T' -> ObsTraceEq T T'.
-Proof.
-  cofix COFIX.
-  intros T T' Eq(*; pfold*).
-  inv Eq.
-  + (* RB: This goal is slightly more involved than it was before. *)
-    (* apply paco2_unfold. *)
-    (* * apply ObsTraceEq_mon. *)
-    (* * apply paco2_mon_bot with ObsTraceEq_gen; auto. *)
-    assumption.
-  + eapply ObsEqTau2.
-    (*right.*) eapply COFIX; auto.
-  + eapply ObsEqTau2.
-    (*left. pfold.*) eapply ObsEqAllSame.
-Qed.
+  Lemma ObsTraceEqRemoveTau1 :
+    forall T T', ObsTraceEq (notfinished Tau T) T' -> ObsTraceEq T T'.
+  Proof.
+    cofix COFIX.
+    intros T T' Eq(*; pfold*).
+    inv Eq.
+    + (* RB: This goal is slightly more involved than it was before. *)
+      (* apply paco2_unfold. *)
+      (* * apply ObsTraceEq_mon. *)
+      (* * apply paco2_mon_bot with ObsTraceEq_gen; auto. *)
+      assumption.
+    + eapply ObsEqTau2.
+      (*right.*) eapply COFIX; auto.
+    + eapply ObsEqTau2.
+      (*left. pfold.*) eapply ObsEqAllSame.
+  Qed.
 
-Lemma ObsTraceEqRemoveTau2 :
-  forall T T', ObsTraceEq T (notfinished Tau T') -> ObsTraceEq T T'.
-Proof.
-  cofix COFIX.
-  intros T T' Eq(*; pfold*).
-  inv Eq.
-  + eapply ObsEqTau1.
-    (*right.*) eapply COFIX.
-    auto.
-  + (* RB: This goal is slightly more involved than it was before. *)
-    (* apply paco2_unfold. *)
-    (* * apply ObsTraceEq_mon. *)
-    (* * apply paco2_mon_bot with ObsTraceEq_gen; auto. *)
-    assumption.
-  + eapply ObsEqTau1. (*left. pfold.*)
-    eapply ObsEqAllSame.
-Qed.
-
-Fixpoint tauN (n : nat) (T : ObsTrace) : ObsTrace := 
-  match n with
-  | O => T
-  | S n' => notfinished Tau (tauN n' T)
-  end.
-
-Lemma EqOut_tauN : forall T' t',
-    Last T' t' ->
-    forall w T, 
-      ObsTraceEq (notfinished (Out w) T) T' ->
-      exists n, T' = tauN n (finished (Out w)) \/ exists  T'', T' = tauN n (notfinished (Out w) T'').
-Proof.
-  intros T' t' HL.
-  induction HL; intros w Tw Eq.
-  - exists 0. left. simpl.
-    inversion Eq.
-  - destruct a'.
-    + inv Eq.
-      * exists 0.
-        right.
-        exists T; simpl; auto.
-      * exists 0.
-        right.
-        exists T; simpl; auto.
-    + inv Eq.
-      destruct (IHHL w Tw HR) as [n [HTau | [T'' HTau]]].
-      * exists (S n).
-        left.
-        simpl.
-        rewrite HTau.
-        auto.
-      * exists (S n).
-        right.
-        simpl.
-        exists T''.
-        rewrite HTau.
-        auto.
-Qed.
-
-Lemma ObsTraceEqApp :
-  forall O1 O1' O2 O2' o1 o1',
-    Last O1 o1 -> Last O1' o1' -> 
-    ObsTraceEq O1 O1' ->
-    ObsTraceEq O2 O2' ->
-    ObsTraceEq (O1^(Some O2)) (O1'^(Some O2')).
-Proof.
-  intros O1 O1' O2 O2' o1 o1' H;
-    revert O1' O2 O2' o1'.
-  induction H as [o1|]; intros O1' O2 O2' o1' Last' Eq1 Eq2.
-  - generalize dependent O2;
-    generalize dependent O2';
-    generalize dependent Eq1.
-    induction Last';
-      intros Eq1 O2' O2 Eq2(*;
-      pfold*).
-    + inversion Eq1; subst; simpl in *; clear Eq1; app_frobber.
-      * destruct a.
-        -- apply ObsEqNow; auto.
-        -- apply ObsEqTau1. (*left. pfold.*) apply ObsEqTau2; auto.
-    + inversion Eq1; subst; simpl in *; clear Eq1.
-      specialize (IHLast' HR O2' O2 Eq2).
-      app_frobber.
-      eapply ObsEqTau2.
+  Lemma ObsTraceEqRemoveTau2 :
+    forall T T', ObsTraceEq T (notfinished Tau T') -> ObsTraceEq T T'.
+  Proof.
+    cofix COFIX.
+    intros T T' Eq(*; pfold*).
+    inv Eq.
+    + eapply ObsEqTau1.
+      (*right.*) eapply COFIX.
       auto.
-  - destruct a'.
-    + destruct (EqOut_tauN O1' o1' Last' w T Eq1) as [n [HTau | [T' HTau]]].
-      * rewrite HTau in *.
-        clear HTau.
-        induction n; simpl in *; subst; app_frobber(*; pfold*).
-        -- apply ObsEqNow.
-           inversion Eq1.
-        -- apply ObsEqTau2.
-           inversion Last'; subst; clear Last'.
-           apply ObsTraceEqRemoveTau2 in Eq1.
-           specialize (IHn H3 Eq1).
-           auto.
-      * rewrite HTau in *.
-        clear HTau.
-        induction n; simpl in *; subst; app_frobber(*; pfold*).
-        -- apply ObsEqNow.
-           inversion Eq1; subst; clear Eq1.
-           (* RB: The following two subgoals become slightly different. *)
-           ++ inversion Last'; subst; clear Last'.
-              (*left.*)
-              eapply IHLast; eauto.
-           ++ inversion Last'; subst; clear Last'.
-              (*left.*)
-              eapply IHLast; eauto.
-        -- inversion Last'; subst; clear Last'.
-           specialize (IHn H3).
-           apply ObsTraceEqRemoveTau2 in Eq1.
-           specialize (IHn Eq1).
-           apply ObsEqTau2.
-           auto.
-    + apply ObsTraceEqRemoveTau1 in Eq1.
-      app_frobber.
-      (* RB: Ditto here, applying IH is now a bit more explicit. *)
-      (*pfold.*) apply ObsEqTau1. (*left.*)
-      eapply IHLast; eauto.
-Qed.
+    + (* RB: This goal is slightly more involved than it was before. *)
+      (* apply paco2_unfold. *)
+      (* * apply ObsTraceEq_mon. *)
+      (* * apply paco2_mon_bot with ObsTraceEq_gen; auto. *)
+      assumption.
+    + eapply ObsEqTau1. (*left. pfold.*)
+      eapply ObsEqAllSame.
+  Qed.
+
+  Fixpoint tauN (n : nat) (T : ObsTrace) : ObsTrace := 
+    match n with
+    | O => T
+    | S n' => notfinished Tau (tauN n' T)
+    end.
+
+  Lemma EqOut_tauN : forall T' t',
+      Last T' t' ->
+      forall w T, 
+        ObsTraceEq (notfinished (Out w) T) T' ->
+        exists n, T' = tauN n (finished (Out w)) \/ exists  T'', T' = tauN n (notfinished (Out w) T'').
+  Proof.
+    intros T' t' HL.
+    induction HL; intros w Tw Eq.
+    - exists 0. left. simpl.
+      inversion Eq.
+    - destruct a'.
+      + inv Eq.
+        * exists 0.
+          right.
+          exists T; simpl; auto.
+        * exists 0.
+          right.
+          exists T; simpl; auto.
+      + inv Eq.
+        destruct (IHHL w Tw HR) as [n [HTau | [T'' HTau]]].
+        * exists (S n).
+          left.
+          simpl.
+          rewrite HTau.
+          auto.
+        * exists (S n).
+          right.
+          simpl.
+          exists T''.
+          rewrite HTau.
+          auto.
+  Qed.
+
+  Lemma ObsTraceEqApp :
+    forall O1 O1' O2 O2' o1 o1',
+      Last O1 o1 -> Last O1' o1' -> 
+      ObsTraceEq O1 O1' ->
+      ObsTraceEq O2 O2' ->
+      ObsTraceEq (O1^(Some O2)) (O1'^(Some O2')).
+  Proof.
+    intros O1 O1' O2 O2' o1 o1' H;
+      revert O1' O2 O2' o1'.
+    induction H as [o1|]; intros O1' O2 O2' o1' Last' Eq1 Eq2.
+    - generalize dependent O2;
+        generalize dependent O2';
+        generalize dependent Eq1.
+      induction Last';
+        intros Eq1 O2' O2 Eq2(*;
+      pfold*). 
+      + inversion Eq1; subst; simpl in *; clear Eq1; app_frobber.
+        * destruct a.
+          -- apply ObsEqNow; auto.
+          -- apply ObsEqTau1. (*left. pfold.*) apply ObsEqTau2; auto.
+      + inversion Eq1; subst; simpl in *; clear Eq1.
+        specialize (IHLast' HR O2' O2 Eq2).
+        app_frobber.
+        eapply ObsEqTau2.
+        auto.
+    - destruct a'.
+      + destruct (EqOut_tauN O1' o1' Last' o T Eq1) as [n [HTau | [T' HTau]]].
+        * rewrite HTau in *.
+          clear HTau.
+          induction n; simpl in *; subst; app_frobber(*; pfold*).
+          -- apply ObsEqNow.
+             inversion Eq1.
+          -- apply ObsEqTau2.
+             inversion Last'; subst; clear Last'.
+             apply ObsTraceEqRemoveTau2 in Eq1.
+             specialize (IHn H3 Eq1).
+             auto.
+        * rewrite HTau in *.
+          clear HTau.
+          induction n; simpl in *; subst; app_frobber(*; pfold*).
+          -- apply ObsEqNow.
+             inversion Eq1; subst; clear Eq1.
+             (* RB: The following two subgoals become slightly different. *)
+             ++ inversion Last'; subst; clear Last'.
+                (*left.*)
+                eapply IHLast; eauto.
+             ++ inversion Last'; subst; clear Last'.
+                (*left.*)
+                eapply IHLast; eauto.
+          -- inversion Last'; subst; clear Last'.
+             specialize (IHn H3).
+             apply ObsTraceEqRemoveTau2 in Eq1.
+             specialize (IHn Eq1).
+             apply ObsEqTau2.
+             auto.
+      + apply ObsTraceEqRemoveTau1 in Eq1.
+        app_frobber.
+        (* RB: Ditto here, applying IH is now a bit more explicit. *)
+        (*pfold.*) apply ObsEqTau1. (*left.*)
+        eapply IHLast; eauto.
+  Qed.
 
 (********************** ObsTrace Prefix *************************)
 
@@ -231,444 +235,443 @@ Definition ObsTracePrefix (OO OO' : TraceOf Observation) : Prop :=
   exists OO'', ObsTraceEq OO OO'' /\ OO' <<== OO'' \/ ObsTraceEq OO' OO'' /\ OO' <<== OO.
  *)
 
-(* The second is a prefix of the first, up to Tau *)
-CoInductive ObsTracePrefix(*_gen R*) : TraceOf Observation -> TraceOf Observation -> Prop :=
-| ObsPreTau1 : forall OO OO'
-                      (HR : (*R*)ObsTracePrefix OO OO' : Prop),
-    ObsTracePrefix(*_gen R*) (notfinished Tau OO) OO'
-| ObsPreTau2 : forall OO OO'
-                      (HR : (*R*)ObsTracePrefix OO OO' : Prop),
-    ObsTracePrefix(*_gen R*) OO (notfinished Tau OO')
-| ObsPreNow : forall w OO OO'
-                      (HR : (*R*)ObsTracePrefix OO OO' : Prop),
-    ObsTracePrefix(*_gen R*) (notfinished (Out w) OO) (notfinished (Out w) OO')
-(*| ObsPreFinishedOut1 : forall w,
-    ObsTracePrefix(*_gen R*) (finished (Out w)) (finished (Out w))
-*)
-| ObsPreFinishedOut2 : forall w OO,
-    ObsTracePrefix(*_gen R*) (notfinished (Out w) OO) (finished (Out w))
-| ObsPreFinishedTau : forall OO,
-    ObsTracePrefix(*_gen R*) OO (finished Tau)
-| ObsPreAllSame : forall OO,
-     ObsTracePrefix(*_gen R*) OO OO.
-Hint Constructors ObsTracePrefix(*_gen*) : core.
+  (* The second is a prefix of the first, up to Tau *)
+  CoInductive ObsTracePrefix(*_gen R*) : TraceOf Observation -> TraceOf Observation -> Prop :=
+  | ObsPreTau1 : forall OO OO'
+                        (HR : (*R*)ObsTracePrefix OO OO' : Prop),
+      ObsTracePrefix(*_gen R*) (notfinished Tau OO) OO'
+  | ObsPreTau2 : forall OO OO'
+                        (HR : (*R*)ObsTracePrefix OO OO' : Prop),
+      ObsTracePrefix(*_gen R*) OO (notfinished Tau OO')
+  | ObsPreNow : forall w OO OO'
+                       (HR : (*R*)ObsTracePrefix OO OO' : Prop),
+      ObsTracePrefix(*_gen R*) (notfinished (Out w) OO) (notfinished (Out w) OO')
+  (*| ObsPreFinishedOut1 : forall w,
+      ObsTracePrefix(*_gen R*) (finished (Out w)) (finished (Out w))
+   *)
+  | ObsPreFinishedOut2 : forall w OO,
+      ObsTracePrefix(*_gen R*) (notfinished (Out w) OO) (finished (Out w))
+  | ObsPreFinishedTau : forall OO,
+      ObsTracePrefix(*_gen R*) OO (finished Tau)
+  | ObsPreAllSame : forall OO,
+      ObsTracePrefix(*_gen R*) OO OO.
+  Hint Constructors ObsTracePrefix(*_gen*) : core.
 
-(* Definition ObsTracePrefix (OO OO' : TraceOf Observation) := *)
-(*   paco2 ObsTracePrefix_gen bot2 OO OO'. *)
-(* Hint Unfold ObsTracePrefix : core. *)
-(* Lemma ObsTracePrefix_mon : monotone2 ObsTracePrefix_gen. Proof. pmonauto. Qed. *)
-(* Hint Resolve ObsTracePrefix_mon : paco. *)
+  (* Definition ObsTracePrefix (OO OO' : TraceOf Observation) := *)
+  (*   paco2 ObsTracePrefix_gen bot2 OO OO'. *)
+  (* Hint Unfold ObsTracePrefix : core. *)
+  (* Lemma ObsTracePrefix_mon : monotone2 ObsTracePrefix_gen. Proof. pmonauto. Qed. *)
+  (* Hint Resolve ObsTracePrefix_mon : paco. *)
 
-Notation "OO' <=_O OO" := (ObsTracePrefix OO OO') (at level 80).
+  Notation "OO' <=_O OO" := (ObsTracePrefix OO OO') (at level 80).
 
-Lemma ObsTracePrefApp' :
-  forall O1 O1' O2 O2' o1 o1',
-    Last O1 o1 -> Last O1' o1' -> 
-    ObsTraceEq O1 O1' ->
-    ObsTracePrefix O2 O2' ->
-    ObsTracePrefix (O1^(Some O2)) (O1'^(Some O2')).
-Proof.
-  intros O1 O1' O2 O2' o1 o1' H;
-    (* I really want SSR... *)
-    revert O1' O2 O2' o1'.
-  induction H as [o1|]; intros O1' O2 O2' o1' Last' Eq Pref.
-  - generalize dependent O2;
-    generalize dependent O2';
-    generalize dependent Eq.
-    induction Last';
-      intros Eq O2' O2 Pref(*; pfold*).
-    + inversion Eq; subst; simpl in *; clear Eq; app_frobber.
-      (* Hint constructors doesn't work for this? *)
-      * destruct a.
-        -- apply ObsPreNow; auto.
-        -- apply ObsPreTau1. (*left. pfold.*) apply ObsPreTau2; auto.
-    + inversion Eq; subst; simpl in *; clear Eq.
-      specialize (IHLast' HR O2' O2 Pref).
-      app_frobber.
-      eapply ObsPreTau2.
-      auto.
-  (* Try by inversion. *)
-  - destruct a'.
-    + destruct (EqOut_tauN O1' o1' Last' w T Eq) as [n [HTau | [T' HTau]]](*;
-        pfold*).
-      * rewrite HTau in *.
-        clear HTau.
-        induction n; simpl in *; subst; app_frobber.
-        -- apply ObsPreNow.
-           inversion Eq. (* This makes me feel strange *)
-        -- apply ObsPreTau2.
-           inversion Last'; subst; clear Last'.
-           apply ObsTraceEqRemoveTau2 in Eq.
-           specialize (IHn H3 Eq).
-           auto.
-      * rewrite HTau in *.
-        clear HTau.
-        induction n; simpl in *; subst; app_frobber.
-        -- apply ObsPreNow.
-           inversion Eq; subst; clear Eq.
-           (* RB: The following two subgoals become slightly different. *)
-           ++ inversion Last'; subst; clear Last'.
-              (*left.*)
-              eapply IHLast; eauto.
-           ++ inversion Last'; subst; clear Last'.
-              (*left.*)
-              eapply IHLast; eauto.
-        -- inversion Last'; subst; clear Last'.
-           specialize (IHn H3).
-           apply ObsTraceEqRemoveTau2 in Eq.
-           specialize (IHn Eq).
-           apply ObsPreTau2.
-           auto.
-    + apply ObsTraceEqRemoveTau1 in Eq.
-      app_frobber.
-      (*pfold.*) apply ObsPreTau1. (*left.*)
-      (* RB: Ditto here, applying IH is now a bit more explicit. *)
-      eapply IHLast; eauto.
-Qed.
+  Lemma ObsTracePrefApp' :
+    forall O1 O1' O2 O2' o1 o1',
+      Last O1 o1 -> Last O1' o1' -> 
+      ObsTraceEq O1 O1' ->
+      ObsTracePrefix O2 O2' ->
+      ObsTracePrefix (O1^(Some O2)) (O1'^(Some O2')).
+  Proof.
+    intros O1 O1' O2 O2' o1 o1' H;
+      (* I really want SSR... *)
+      revert O1' O2 O2' o1'.
+    induction H as [o1|]; intros O1' O2 O2' o1' Last' Eq Pref.
+    - generalize dependent O2;
+        generalize dependent O2';
+        generalize dependent Eq.
+      induction Last';
+        intros Eq O2' O2 Pref(*; pfold*).
+      + inversion Eq; subst; simpl in *; clear Eq; app_frobber.
+        (* Hint constructors doesn't work for this? *)
+        * destruct a.
+          -- apply ObsPreNow; auto.
+          -- apply ObsPreTau1. (*left. pfold.*) apply ObsPreTau2; auto.
+      + inversion Eq; subst; simpl in *; clear Eq.
+        specialize (IHLast' HR O2' O2 Pref).
+        app_frobber.
+        eapply ObsPreTau2.
+        auto.
+    (* Try by inversion. *)
+    - destruct a'.
+      + destruct (EqOut_tauN O1' o1' Last' o T Eq) as [n [HTau | [T' HTau]]](*;
+        pfold*). 
+        * rewrite HTau in *.
+          clear HTau.
+          induction n; simpl in *; subst; app_frobber.
+          -- apply ObsPreNow.
+             inversion Eq. (* This makes me feel strange *)
+          -- apply ObsPreTau2.
+             inversion Last'; subst; clear Last'.
+             apply ObsTraceEqRemoveTau2 in Eq.
+             specialize (IHn H3 Eq).
+             auto.
+        * rewrite HTau in *.
+          clear HTau.
+          induction n; simpl in *; subst; app_frobber.
+          -- apply ObsPreNow.
+             inversion Eq; subst; clear Eq.
+             (* RB: The following two subgoals become slightly different. *)
+             ++ inversion Last'; subst; clear Last'.
+                (*left.*)
+                eapply IHLast; eauto.
+             ++ inversion Last'; subst; clear Last'.
+                (*left.*)
+                eapply IHLast; eauto.
+          -- inversion Last'; subst; clear Last'.
+             specialize (IHn H3).
+             apply ObsTraceEqRemoveTau2 in Eq.
+             specialize (IHn Eq).
+             apply ObsPreTau2.
+             auto.
+      + apply ObsTraceEqRemoveTau1 in Eq.
+        app_frobber.
+        (*pfold.*) apply ObsPreTau1. (*left.*)
+        (* RB: Ditto here, applying IH is now a bit more explicit. *)
+        eapply IHLast; eauto.
+  Qed.
+  
+  Lemma ObsTracePrefix_refl : forall OO, ObsTracePrefix OO OO.
+  Proof.
+    cofix CH.
+    intros [o | o OO](*; pfold*).
+    - constructor. 
+    - destruct o as [w |].
+      + apply ObsPreNow. now auto.
+      + apply ObsPreTau1. (*left. pfold.*) apply ObsPreTau2. now auto.
+  Qed.
 
-Lemma ObsTracePrefix_refl : forall OO, ObsTracePrefix OO OO.
-Proof.
-  cofix CH.
-  intros [o | o OO](*; pfold*).
-  - constructor. 
-  - destruct o as [w |].
-    + apply ObsPreNow. now auto.
-    + apply ObsPreTau1. (*left. pfold.*) apply ObsPreTau2. now auto.
-Qed.
+  Lemma ObsTracePrefRemoveTau1 :
+    forall T T', (notfinished Tau T) <=_O T' -> T <=_O T'.
+  Proof.
+    cofix COFIX.
+    intros T T' Pref(*; pfold*).
+    inv Pref.
+    + constructor. (*right.*) apply COFIX. auto.
+    + (* RB: Some base cases like this need a little more work than before. *)
+      (* apply paco2_unfold. *)
+      (* * auto with paco. *)
+      (* * eapply paco2_mon_bot; eauto with paco. *)
+      assumption.
+    + constructor. (*left.
+                     eapply paco2_mon_bot with ObsTracePrefix_gen; [| auto].*)
+      apply ObsTracePrefix_refl.
+  Qed.
+  
+  Lemma ObsTracePrefRemoveTau2 :
+    forall T T', T <=_O (notfinished Tau T') -> T <=_O T'.
+  Proof.
+    cofix COFIX.
+    intros T T' Pref.
+    inv Pref.
+    + assumption.
+    + constructor. apply COFIX. auto.
+    + constructor. 
+    + constructor. 
+      apply ObsTracePrefix_refl.
+  Qed.
 
-Lemma ObsTracePrefRemoveTau1 :
-  forall T T', (notfinished Tau T) <=_O T' -> T <=_O T'.
-Proof.
-  cofix COFIX.
-  intros T T' Pref(*; pfold*).
-  inv Pref.
-  + constructor. (*right.*) apply COFIX. auto.
-  + (* RB: Some base cases like this need a little more work than before. *)
-    (* apply paco2_unfold. *)
-    (* * auto with paco. *)
-    (* * eapply paco2_mon_bot; eauto with paco. *)
-    assumption.
-  + constructor. (*left.
-    eapply paco2_mon_bot with ObsTracePrefix_gen; [| auto].*)
-    apply ObsTracePrefix_refl.
-Qed.
+  Lemma ObsTracePrefFinished: forall OO, OO <=_O finished Tau -> OO ~=_O finished Tau.
+  Proof.
+    cofix COFIX. 
+    intros. 
+    inv H.
+    - constructor. apply COFIX; auto.
+    - constructor. 
+    - constructor. 
+  Qed.
 
-Lemma ObsTracePrefRemoveTau2 :
-  forall T T', T <=_O (notfinished Tau T') -> T <=_O T'.
-Proof.
-  cofix COFIX.
-  intros T T' Pref.
-  inv Pref.
-  + assumption.
-  + constructor. apply COFIX. auto.
-  + constructor. 
-  + constructor. 
-    apply ObsTracePrefix_refl.
-Qed.
+  (** Alternative definition of ObsTraceEq. *)
+  
+  Definition ObsTraceEq' OO OO' : Prop :=  ObsTracePrefix OO OO' /\ ObsTracePrefix OO' OO. 
 
-Lemma ObsTracePrefFinished: forall OO, OO <=_O finished Tau -> OO ~=_O finished Tau.
-Proof.
-  cofix COFIX. 
-  intros. 
-  inv H.
-  - constructor. apply COFIX; auto.
-  - constructor. 
-  - constructor. 
-Qed.
+  Lemma OTE'E: forall T T', ObsTraceEq' T T' -> ObsTraceEq T T'. 
+  Proof.
+    cofix COFIX.
+    intros T T' [H1 H2].
+    inv H1; inv H2; try apply ObsEqAllSame.  
+    - apply ObsTracePrefRemoveTau1 in HR.  apply ObsTracePrefRemoveTau1 in HR0.  
+      constructor. constructor. apply COFIX; split; auto.
+    - constructor.  apply COFIX; split;  auto. 
+    - constructor. apply COFIX; split; auto.
+    - apply ObsTracePrefRemoveTau2 in HR. apply ObsTracePrefRemoveTau2 in HR0. 
+      constructor. constructor. apply COFIX; split; auto.
+    - constructor.
+      apply ObsTracePrefFinished in HR. apply ObsTraceEq_sym. auto.
+    - constructor. apply COFIX; split; auto. 
+    - constructor. 
+      apply ObsTracePrefFinished in HR. auto.
+  Qed.
 
-(** Alternative definition of ObsTraceEq. *)
+  Lemma OTEE'1 : forall T T', ObsTraceEq T T' -> ObsTracePrefix T T'. 
+  Proof.
+    cofix COFIX. 
+    intros. 
+    inv H; constructor; eauto.  
+  Qed.
 
-Definition ObsTraceEq' OO OO' : Prop :=  ObsTracePrefix OO OO' /\ ObsTracePrefix OO' OO. 
-
-Lemma OTE'E: forall T T', ObsTraceEq' T T' -> ObsTraceEq T T'. 
-Proof.
-  cofix COFIX.
-  intros T T' [H1 H2].
-  inv H1; inv H2; try apply ObsEqAllSame.  
-  - apply ObsTracePrefRemoveTau1 in HR.  apply ObsTracePrefRemoveTau1 in HR0.  
-    constructor. constructor. apply COFIX; split; auto.
-  - constructor.  apply COFIX; split;  auto. 
-  - constructor. apply COFIX; split; auto.
-  - apply ObsTracePrefRemoveTau2 in HR. apply ObsTracePrefRemoveTau2 in HR0. 
-    constructor. constructor. apply COFIX; split; auto.
-  - constructor.
-    apply ObsTracePrefFinished in HR. apply ObsTraceEq_sym. auto.
-  - constructor. apply COFIX; split; auto. 
-  - constructor. 
-    apply ObsTracePrefFinished in HR. auto.
-Qed.
-
-Lemma OTEE'1 : forall T T', ObsTraceEq T T' -> ObsTracePrefix T T'. 
-Proof.
-  cofix COFIX. 
-  intros. 
-  inv H; constructor; eauto.  
-Qed.
-
-Lemma OTEE'2 : forall T T', ObsTraceEq T T' -> ObsTracePrefix T' T. 
-Proof.
-  cofix COFIX. 
-  intros. 
-  inv H; constructor; eauto.  
-Qed.
-
-Lemma OTEE': forall T T', ObsTraceEq T T' -> ObsTraceEq' T T'. 
-Proof.
-  intros.
-  split.
-  - apply OTEE'1; auto. 
-  - apply OTEE'2;  auto. 
-Qed.
-
-
-(********************** Relationship betweeen Traces and ObsTraces  *************************)
+  Lemma OTEE'2 : forall T T', ObsTraceEq T T' -> ObsTracePrefix T' T. 
+  Proof.
+    cofix COFIX. 
+    intros. 
+    inv H; constructor; eauto.  
+  Qed.
+  
+  Lemma OTEE': forall T T', ObsTraceEq T T' -> ObsTraceEq' T T'. 
+  Proof.
+    intros.
+    split.
+    - apply OTEE'1; auto. 
+    - apply OTEE'2;  auto. 
+  Qed.
 
 
-Lemma TraceEqImpliesObsTraceEq :
-  forall O O',
-    O ~= O' ->
-    ObsTraceEq O O'.
-Proof.
-  cofix COFIX. intros O O' H(*; pfold*). inv H.
-  - constructor.
-  - destruct a.
-    + constructor. auto.
-    + constructor. (*left. pfold.*) constructor. auto.
-Qed.
+  (********************** Relationship betweeen Traces and ObsTraces  *************************)
 
-Lemma ObsTraceEqImpliesPrefix :
-  forall O O',
-    ObsTraceEq O O' ->
-    O <=_O O'.
-Proof.
-  cofix COFIX. intros O O' H. (*pfold.*)
-  inv H; constructor; (*right;*) apply COFIX; auto.
-Qed.
 
-    
-Lemma ObsPrefOverEq :
-  forall O1 O1' O2,
-    O1 ~= O1' ->
-    O1 <=_O O2 ->
-    O1' <=_O O2.
-Proof.
-  cofix COFIX. intros O1 O1' O2 H H0(*; pfold*). inv H.
-  - assumption.
+  Lemma TraceEqImpliesObsTraceEq :
+    forall O O',
+      O ~= O' ->
+      ObsTraceEq O O'.
+  Proof.
+    cofix COFIX. intros O O' H(*; pfold*). inv H.
+    - constructor.
+    - destruct a.
+      + constructor. auto.
+      + constructor. (*left. pfold.*) constructor. auto.
+  Qed.
+
+  Lemma ObsTraceEqImpliesPrefix :
+    forall O O',
+      ObsTraceEq O O' ->
+      O <=_O O'.
+  Proof.
+    cofix COFIX. intros O O' H. (*pfold.*)
+    inv H; constructor; (*right;*) apply COFIX; auto.
+  Qed.
+
+  Lemma ObsPrefOverEq :
+    forall O1 O1' O2,
+      O1 ~= O1' ->
+      O1 <=_O O2 ->
+      O1' <=_O O2.
+  Proof.
+    cofix COFIX. intros O1 O1' O2 H H0(*; pfold*). inv H.
+    - assumption.
     (* apply paco2_unfold. *)
     (* + auto with paco. *)
     (* + eapply paco2_mon_bot; eauto with paco. *)
-  - destruct a.
-    + inv H0.
-      * constructor. (*right.*)
-        apply (COFIX (notfinished (Out w) T1) (notfinished (Out w) T2) OO).
-        -- (*pfold.*) constructor. auto.
-        -- auto.
-      * constructor. (*right.*) apply (COFIX T1 T2 OO); auto.
-      * constructor.
-        (* left. *)
-        (* apply paco2_mon_bot with ObsTracePrefix_gen; [| auto]. *)
-        apply ObsTraceEqImpliesPrefix. apply TraceEqImpliesObsTraceEq in H1.
-        apply ObsTraceEq_sym. auto.
-    + constructor. (*right.*) apply (COFIX T1 T2 O2); auto. apply ObsTracePrefRemoveTau1. auto.
-Qed.
+    - destruct a.
+      + inv H0.
+        * constructor. (*right.*)
+          apply (COFIX (notfinished (Out o) T1) (notfinished (Out o) T2) OO).
+          -- (*pfold.*) constructor. auto.
+          -- auto.
+        * constructor. (*right.*) apply (COFIX T1 T2 OO); auto.
+        * constructor.
+          (* left. *)
+          (* apply paco2_mon_bot with ObsTracePrefix_gen; [| auto]. *)
+          apply ObsTraceEqImpliesPrefix. apply TraceEqImpliesObsTraceEq in H1.
+          apply ObsTraceEq_sym. auto.
+      + constructor. (*right.*) apply (COFIX T1 T2 O2); auto. apply ObsTracePrefRemoveTau1. auto.
+  Qed.
 
-Lemma ObsPrefOverEq2 :
-  forall O1 O2 O2',
-    O2 ~= O2' ->
-    O1 <=_O O2 ->
-    O1 <=_O O2'.
-Proof.
-  cofix COFIX. intros O1 O2 O2' H H0. inv H.
-  - assumption.
-  - destruct a.
-    + inv H0.
-      * constructor.
-        apply (COFIX OO' (notfinished (Out w) T1) (notfinished (Out w) T2)).
-        -- constructor. auto.
-        -- auto.
-      * constructor. apply (COFIX OO' T1 T2); auto.
-      * constructor.
-      * constructor.
-      * constructor. apply ObsTraceEqImpliesPrefix. apply TraceEqImpliesObsTraceEq. auto.
-    + constructor. apply (COFIX O1 T1 T2); auto. apply ObsTracePrefRemoveTau2. auto.
-Qed.
+  Lemma ObsPrefOverEq2 :
+    forall O1 O2 O2',
+      O2 ~= O2' ->
+      O1 <=_O O2 ->
+      O1 <=_O O2'.
+  Proof.
+    cofix COFIX. intros O1 O2 O2' H H0. inv H.
+    - assumption.
+    - destruct a.
+      + inv H0.
+        * constructor.
+          apply (COFIX OO' (notfinished (Out o) T1) (notfinished (Out o) T2)).
+          -- constructor. auto.
+          -- auto.
+        * constructor. apply (COFIX OO' T1 T2); auto.
+        * constructor.
+        * constructor.
+        * constructor. apply ObsTraceEqImpliesPrefix. apply TraceEqImpliesObsTraceEq. auto.
+      + constructor. apply (COFIX O1 T1 T2); auto. apply ObsTracePrefRemoveTau2. auto.
+  Qed.
 
-Lemma ObsEqOverEq :
-  forall O1 O1' O2,
-    O1 ~= O1' ->
-    ObsTraceEq O1 O2 ->
-    ObsTraceEq O1' O2.
-Proof.
-  cofix COFIX. intros O1 O1' O2 H H0(*; pfold*). inv H.
-  - assumption.
+  Lemma ObsEqOverEq :
+    forall O1 O1' O2,
+      O1 ~= O1' ->
+      ObsTraceEq O1 O2 ->
+      ObsTraceEq O1' O2.
+  Proof.
+    cofix COFIX. intros O1 O1' O2 H H0(*; pfold*). inv H.
+    - assumption.
     (* apply paco2_unfold. *)
     (* * auto with paco. *)
     (* * eapply paco2_mon_bot; eauto with paco. *)
-  - destruct a.
-    + inv H0.
-      * constructor. (*right.*)
-        apply (COFIX (notfinished (Out w) T1) (notfinished (Out w) T2) OO').
-        -- (*pfold.*) constructor. auto.
-        -- auto.
-      * constructor. (*right.*) apply (COFIX T1 T2 OO'); auto.
-      * constructor.
-        (* left. *)
-        (* apply paco2_mon_bot with ObsTraceEq_gen; [| auto]. *)
-        apply ObsTraceEq_sym. apply TraceEqImpliesObsTraceEq. auto.
-    + constructor. (*right.*) apply (COFIX T1 T2 O2); auto. apply ObsTraceEqRemoveTau1. auto.
-Qed.
+    - destruct a.
+      + inv H0.
+        * constructor. (*right.*)
+          apply (COFIX (notfinished (Out o) T1) (notfinished (Out o) T2) OO').
+          -- (*pfold.*) constructor. auto.
+          -- auto.
+        * constructor. (*right.*) apply (COFIX T1 T2 OO'); auto.
+        * constructor.
+          (* left. *)
+          (* apply paco2_mon_bot with ObsTraceEq_gen; [| auto]. *)
+          apply ObsTraceEq_sym. apply TraceEqImpliesObsTraceEq. auto.
+      + constructor. (*right.*) apply (COFIX T1 T2 O2); auto. apply ObsTraceEqRemoveTau1. auto.
+  Qed.
 
 (***** Taking ObsTraces from traces and runs *****)
 
-CoFixpoint ObsTraceOfM (M: MTrace) : ObsTrace :=
-  match M with
-  | finished m =>
-    finished Tau
-  | notfinished m M' =>
-    let (m', O) := step m in
-    notfinished O (ObsTraceOfM M')
-  end.
+(*  CoFixpoint ObsTraceOfM (M: MTrace) : ObsTrace :=
+    match M with
+    | finished m =>
+      finished Tau
+    | notfinished m M' =>
+      let (m', O) := step m in
+      notfinished O (ObsTraceOfM M')
+    end.
+  
+  CoFixpoint ObsTraceOf (MP: MPTrace) : ObsTrace := 
+    match MP with
+    | finished mp =>
+      finished Tau
+    | notfinished mp MP' =>
+      let (m', O) := step (ms mp) in
+      notfinished O (ObsTraceOf MP')
+    end.
 
-CoFixpoint ObsTraceOf (MP: MPTrace) : ObsTrace := 
-  match MP with
-  | finished mp =>
-    finished Tau
-  | notfinished mp MP' =>
-    let (m', O) := step (ms mp) in
-    notfinished O (ObsTraceOf MP')
-  end.
+  Definition ObsOfMP (MPO : MPTrace') : TraceOf Observation :=
+    mapTrace snd MPO.
 
-Definition ObsOfMP (MPO : MPTrace') : TraceOf Observation :=
-  mapTrace snd MPO.
+  Definition ObsOfM (MO : MTrace') : TraceOf Observation :=
+    mapTrace snd MO.
 
-Definition ObsOfM (MO : MTrace') : TraceOf Observation :=
-  mapTrace snd MO.
+  (***** Lemmas about JoinInclusive on ObsTraces *****)
 
-(***** Lemmas about JoinInclusive on ObsTraces *****)
+  Definition ObsOfMPJoin :
+    forall MPO MPO',
+      ObsOfMP (MPO ^^ MPO') ~= (ObsOfMP MPO ^^ ObsOfMP MPO').
+  Proof.
+    unfold ObsOfMP. apply MapOverJoin.
+  Qed.
 
-Definition ObsOfMPJoin :
-  forall MPO MPO',
-    ObsOfMP (MPO ^^ MPO') ~= (ObsOfMP MPO ^^ ObsOfMP MPO').
-Proof.
-  unfold ObsOfMP. apply MapOverJoin.
-Qed.
-
-Definition ObsOfMJoin :
-  forall MO MO',
-    ObsOfM (MO ^^ MO') ~= (ObsOfM MO ^^ ObsOfM MO').
-Proof.
-  unfold ObsOfM. apply MapOverJoin.
-Qed.
-
-Lemma ObsEqJoin :
-  forall O1 O1' O2 O2' o1 o1',
-    Last O1 o1 ->
-    Last O1' o1' ->
-    O1 ~=_O O1' ->
-    O2 ~=_O O2' ->
-    (O1 ^^ O2) ~=_O (O1' ^^ O2').
-Proof.
+  Definition ObsOfMJoin :
+    forall MO MO',
+      ObsOfM (MO ^^ MO') ~= (ObsOfM MO ^^ ObsOfM MO').
+  Proof.
+    unfold ObsOfM. apply MapOverJoin.
+  Qed.
+*)
+  Lemma ObsEqJoin :
+    forall O1 O1' O2 O2' o1 o1',
+      Last O1 o1 ->
+      Last O1' o1' ->
+      O1 ~=_O O1' ->
+      O2 ~=_O O2' ->
+      (O1 ^^ O2) ~=_O (O1' ^^ O2').
+  Proof.
     intros O1 O1' O2 O2' o1 o1' H;
-    revert O1' O2 O2' o1'.
-  induction H as [o1|]; intros O1' O2 O2' o1' Last' Eq1 Eq2.
-  - generalize dependent O2;
-    generalize dependent O2';
-    generalize dependent Eq1.
-    induction Last';
-      intros Eq1 O2' O2 Eq2(*;
-      pfold*).
-    + inversion Eq1; subst; simpl in *; clear Eq1; join_frobber.
-      destruct O2; destruct O2'; auto.
-    + inversion Eq1; subst; simpl in *; clear Eq1.
-      specialize (IHLast' HR O2' O2 Eq2).
-      join_frobber.
-      eapply ObsEqTau2.
-      auto.
-  - destruct a'.
-    + destruct (EqOut_tauN O1' o1' Last' w T Eq1) as [n [HTau | [T' HTau]]].
-      * rewrite HTau in *.
-        clear HTau.
-        induction n; simpl in *; subst; join_frobber.
-        -- inversion Eq1.
-        -- apply ObsEqTau2.
-           inversion Last'; subst; clear Last'.
-           apply ObsTraceEqRemoveTau2 in Eq1.
-           specialize (IHn H3 Eq1).
-           auto.
-      * rewrite HTau in *.
-        clear HTau.
-        induction n; simpl in *; subst; join_frobber.
-        -- apply ObsEqNow.
-           inversion Eq1; subst; clear Eq1.
-           ++ inversion Last'; subst; clear Last'.
-              eapply IHLast; eauto.
-           ++ inversion Last'; subst; clear Last'.
-              eapply IHLast; eauto.
-        -- inversion Last'; subst; clear Last'.
-           specialize (IHn H3).
-           apply ObsTraceEqRemoveTau2 in Eq1.
-           specialize (IHn Eq1).
-           apply ObsEqTau2.
-           auto.
-    + apply ObsTraceEqRemoveTau1 in Eq1.
-      join_frobber. apply ObsEqTau1.
-      eapply IHLast; eauto.
-Qed.
+      revert O1' O2 O2' o1'.
+    induction H as [o1|]; intros O1' O2 O2' o1' Last' Eq1 Eq2.
+    - generalize dependent O2;
+        generalize dependent O2';
+        generalize dependent Eq1.
+      induction Last';
+        intros Eq1 O2' O2 Eq2(*;
+      pfold*). 
+      + inversion Eq1; subst; simpl in *; clear Eq1; join_frobber.
+        destruct O2; destruct O2'; auto.
+      + inversion Eq1; subst; simpl in *; clear Eq1.
+        specialize (IHLast' HR O2' O2 Eq2).
+        join_frobber.
+        eapply ObsEqTau2.
+        auto.
+    - destruct a'.
+      + destruct (EqOut_tauN O1' o1' Last' o T Eq1) as [n [HTau | [T' HTau]]].
+        * rewrite HTau in *.
+          clear HTau.
+          induction n; simpl in *; subst; join_frobber.
+          -- inversion Eq1.
+          -- apply ObsEqTau2.
+             inversion Last'; subst; clear Last'.
+             apply ObsTraceEqRemoveTau2 in Eq1.
+             specialize (IHn H3 Eq1).
+             auto.
+        * rewrite HTau in *.
+          clear HTau.
+          induction n; simpl in *; subst; join_frobber.
+          -- apply ObsEqNow.
+             inversion Eq1; subst; clear Eq1.
+             ++ inversion Last'; subst; clear Last'.
+                eapply IHLast; eauto.
+             ++ inversion Last'; subst; clear Last'.
+                eapply IHLast; eauto.
+          -- inversion Last'; subst; clear Last'.
+             specialize (IHn H3).
+             apply ObsTraceEqRemoveTau2 in Eq1.
+             specialize (IHn Eq1).
+             apply ObsEqTau2.
+             auto.
+      + apply ObsTraceEqRemoveTau1 in Eq1.
+        join_frobber. apply ObsEqTau1.
+        eapply IHLast; eauto.
+  Qed.
 
 
-Lemma ObsPrefJoin :
-  forall O1 O1' O2 O2' o1 o1',
-    Last O1 o1 ->
-    Last O1' o1' ->
-    O1 ~=_O O1' ->
-    O2 <=_O O2' ->
-    (O1 ^^ O2) <=_O (O1' ^^ O2').
-Proof.
+  Lemma ObsPrefJoin :
+    forall O1 O1' O2 O2' o1 o1',
+      Last O1 o1 ->
+      Last O1' o1' ->
+      O1 ~=_O O1' ->
+      O2 <=_O O2' ->
+      (O1 ^^ O2) <=_O (O1' ^^ O2').
+  Proof.
     intros O1 O1' O2 O2' o1 o1' H;
-    revert O1' O2 O2' o1'.
-  induction H as [o1|]; intros O1' O2 O2' o1' Last' Eq Pref.
-  - generalize dependent O2;
-    generalize dependent O2';
-    generalize dependent Eq.
-    induction Last';
-      intros Eq O2' O2 Pref.
-    + inversion Eq; subst; simpl in *; clear Eq; join_frobber.
-      destruct O2; destruct O2'; auto.
-    + inversion Eq; subst; simpl in *; clear Eq.
-      specialize (IHLast' HR O2' O2 Pref).
-      join_frobber.
-      eapply ObsPreTau1.
-      auto.
-  - destruct a'.
-    + destruct (EqOut_tauN O1' o1' Last' w T Eq) as [n [HTau | [T' HTau]]].
-      * rewrite HTau in *.
-        clear HTau.
-        induction n; simpl in *; subst; join_frobber.
-        -- inversion Eq.
-        -- apply ObsPreTau1.
-           inversion Last'; subst; clear Last'.
-           apply ObsTraceEqRemoveTau2 in Eq.
-           specialize (IHn H3 Eq).
-           auto.
-      * rewrite HTau in *.
-        clear HTau.
-        induction n; simpl in *; subst; join_frobber.
-        -- apply ObsPreNow.
-           inversion Eq; subst; clear Eq.
-           ++ inversion Last'; subst; clear Last'.
-              eapply IHLast; eauto.
-           ++ inversion Last'; subst; clear Last'.
-              eapply IHLast; eauto.
-        -- inversion Last'; subst; clear Last'.
-           specialize (IHn H3).
-           apply ObsTraceEqRemoveTau2 in Eq.
-           specialize (IHn Eq).
-           apply ObsPreTau1.
-           auto.
-    + apply ObsTraceEqRemoveTau1 in Eq.
-      join_frobber. apply ObsPreTau2.
-      eapply IHLast; eauto.
-Qed.
+      revert O1' O2 O2' o1'.
+    induction H as [o1|]; intros O1' O2 O2' o1' Last' Eq Pref.
+    - generalize dependent O2;
+        generalize dependent O2';
+        generalize dependent Eq.
+      induction Last';
+        intros Eq O2' O2 Pref.
+      + inversion Eq; subst; simpl in *; clear Eq; join_frobber.
+        destruct O2; destruct O2'; auto.
+      + inversion Eq; subst; simpl in *; clear Eq.
+        specialize (IHLast' HR O2' O2 Pref).
+        join_frobber.
+        eapply ObsPreTau1.
+        auto.
+    - destruct a'.
+      + destruct (EqOut_tauN O1' o1' Last' o T Eq) as [n [HTau | [T' HTau]]].
+        * rewrite HTau in *.
+          clear HTau.
+          induction n; simpl in *; subst; join_frobber.
+          -- inversion Eq.
+          -- apply ObsPreTau1.
+             inversion Last'; subst; clear Last'.
+             apply ObsTraceEqRemoveTau2 in Eq.
+             specialize (IHn H3 Eq).
+             auto.
+        * rewrite HTau in *.
+          clear HTau.
+          induction n; simpl in *; subst; join_frobber.
+          -- apply ObsPreNow.
+             inversion Eq; subst; clear Eq.
+             ++ inversion Last'; subst; clear Last'.
+                eapply IHLast; eauto.
+             ++ inversion Last'; subst; clear Last'.
+                eapply IHLast; eauto.
+          -- inversion Last'; subst; clear Last'.
+             specialize (IHn H3).
+             apply ObsTraceEqRemoveTau2 in Eq.
+             specialize (IHn Eq).
+             apply ObsPreTau1.
+             auto.
+      + apply ObsTraceEqRemoveTau1 in Eq.
+        join_frobber. apply ObsPreTau2.
+        eapply IHLast; eauto.
+  Qed.
 
 (*
 Lemma MPRunPrefRun :
@@ -827,3 +830,4 @@ Qed.
 
  *)
 
+End ObsTrace.
